BV/ClassAdd.thy
@@ -1,0 +1,829 @@
+(*  Title: JinjaDCI/BV/ClassAdd.thy
+    Author:     Susannah Mansky
+    2018, UIUC
+*)
+(* Preservation of various properties when adding a class to a program *)
+
+theory ClassAdd
+imports BVConform
+begin
+
+(* HERE: MOVE *)
+lemma err_mono: "A \<subseteq> B \<Longrightarrow> err A \<subseteq> err B"
+ by(unfold err_def) auto
+
+lemma opt_mono: "A \<subseteq> B \<Longrightarrow> opt A \<subseteq> opt B"
+ by(unfold opt_def) auto
+
+(* HERE: MOVE ! ! *)
+lemma Object_fields:
+ "\<lbrakk> P \<turnstile> Object has_fields FDTs; C \<noteq> Object \<rbrakk> \<Longrightarrow> map_of FDTs (F,C) = None"
+ by(drule Fields.cases, auto simp: map_of_reinsert_neq_None)
+
+(* HERE: MOVE! *)
+lemma has_fields_is_class_Object:
+ "P \<turnstile> D has_fields FDTs \<Longrightarrow> is_class P Object"
+ by(induct rule: Fields.induct; simp add: is_class_def)
+
+(* HERE: MOVE! *)
+lemma sees_methods_is_class_Object:
+ "P \<turnstile> D sees_methods Mm \<Longrightarrow> is_class P Object"
+ by(induct rule: Methods.induct; simp add: is_class_def)
+
+(******************)
+
+abbreviation class_add :: "jvm_prog \<Rightarrow> jvm_method cdecl \<Rightarrow> jvm_prog" where
+"class_add P cd \<equiv> cd#P"
+
+lemma class_add_has_fields:
+assumes fs: "P \<turnstile> D has_fields FDTs" and nc: "\<not>is_class P C"
+shows "class_add P (C, cdec) \<turnstile> D has_fields FDTs"
+using assms
+proof(induct rule: Fields.induct)
+  case (has_fields_Object D fs ms FDTs)
+  from has_fields_is_class_Object[OF fs] nc have "C \<noteq> Object" by fast
+  with has_fields_Object show ?case
+   by(auto simp: class_def fun_upd_apply intro!: TypeRel.has_fields_Object)
+next
+  case rec: (has_fields_rec C1 D fs ms FDTs FDTs')
+  with has_fields_is_class have [simp]: "D \<noteq> C" by auto
+  with rec have "C1 \<noteq> C" by(clarsimp simp: is_class_def)
+  with rec show ?case
+   by(auto simp: class_def fun_upd_apply intro: TypeRel.has_fields_rec)
+qed
+
+lemma class_add_has_fields_rev:
+ "\<lbrakk> class_add P (C, cdec) \<turnstile> D has_fields FDTs; \<not>P \<turnstile> D \<preceq>\<^sup>* C \<rbrakk>
+ \<Longrightarrow> P \<turnstile> D has_fields FDTs"
+proof(induct rule: Fields.induct)
+  case (has_fields_Object D fs ms FDTs)
+  then show ?case by(auto simp: class_def fun_upd_apply intro!: TypeRel.has_fields_Object)
+next
+  case rec: (has_fields_rec C1 D fs ms FDTs FDTs')
+  then have sub1: "P \<turnstile> C1 \<prec>\<^sup>1 D"
+   by(auto simp: class_def fun_upd_apply intro!: subcls1I split: if_split_asm)
+  with rec.prems have cls: "\<not> P \<turnstile> D \<preceq>\<^sup>* C" by (meson converse_rtrancl_into_rtrancl)
+  with cls rec show ?case
+   by(auto simp: class_def fun_upd_apply
+           intro: TypeRel.has_fields_rec split: if_split_asm)
+qed
+
+lemma class_add_has_field:
+assumes "P \<turnstile> C\<^sub>0 has F,b:T in D" and "\<not> is_class P C"
+shows "class_add P (C, cdec) \<turnstile> C\<^sub>0 has F,b:T in D"
+using assms by(auto simp: has_field_def dest!: class_add_has_fields[of P C\<^sub>0])
+
+lemma class_add_has_field_rev:
+assumes has: "class_add P (C, cdec) \<turnstile> C\<^sub>0 has F,b:T in D"
+ and ncp: "\<And>D'. P \<turnstile> C\<^sub>0 \<preceq>\<^sup>* D' \<Longrightarrow> D' \<noteq> C"
+shows "P \<turnstile> C\<^sub>0 has F,b:T in D"
+using assms by(auto simp add: has_field_def dest!: class_add_has_fields_rev)
+
+lemma class_add_sees_field:
+assumes "P \<turnstile> C\<^sub>0 sees F,b:T in D" and "\<not> is_class P C"
+shows "class_add P (C, cdec) \<turnstile> C\<^sub>0 sees F,b:T in D"
+using assms by(auto simp: sees_field_def dest!: class_add_has_fields[of P C\<^sub>0])
+
+lemma class_add_sees_field_rev:
+assumes has: "class_add P (C, cdec) \<turnstile> C\<^sub>0 sees F,b:T in D"
+ and ncp: "\<And>D'. P \<turnstile> C\<^sub>0 \<preceq>\<^sup>* D' \<Longrightarrow> D' \<noteq> C"
+shows "P \<turnstile> C\<^sub>0 sees F,b:T in D"
+using assms by(auto simp add: sees_field_def dest!: class_add_has_fields_rev)
+
+lemma class_add_field:
+assumes fd: "P \<turnstile> C\<^sub>0 sees F,b:T in D" and "\<not> is_class P C"
+shows "field P C\<^sub>0 F = field (class_add P (C, cdec)) C\<^sub>0 F"
+using class_add_sees_field[OF assms, of cdec] fd by simp
+
+lemma class_add_sees_methods:
+assumes ms: "P \<turnstile> D sees_methods Mm" and nc: "\<not>is_class P C"
+shows "class_add P (C, cdec) \<turnstile> D sees_methods Mm"
+using assms
+proof(induct rule: Methods.induct)
+  case (sees_methods_Object D fs ms Mm)
+  from sees_methods_is_class_Object[OF ms] nc have "C \<noteq> Object" by fast
+  with sees_methods_Object show ?case
+   by(auto simp: class_def fun_upd_apply intro!: TypeRel.sees_methods_Object)
+next
+  case rec: (sees_methods_rec C1 D fs ms Mm Mm')
+  with sees_methods_is_class have [simp]: "D \<noteq> C" by auto
+  with rec have "C1 \<noteq> C" by(clarsimp simp: is_class_def)
+  with rec show ?case
+   by(auto simp: class_def fun_upd_apply intro: TypeRel.sees_methods_rec)
+qed
+
+lemma class_add_sees_methods_rev:
+ "\<lbrakk> class_add P (C, cdec) \<turnstile> D sees_methods Mm;
+    \<And>D'. P \<turnstile> D \<preceq>\<^sup>* D' \<Longrightarrow> D' \<noteq> C \<rbrakk>
+ \<Longrightarrow> P \<turnstile> D sees_methods Mm"
+proof(induct rule: Methods.induct)
+  case (sees_methods_Object D fs ms Mm)
+  then show ?case
+   by(auto simp: class_def fun_upd_apply intro!: TypeRel.sees_methods_Object)
+next
+  case rec: (sees_methods_rec C1 D fs ms Mm Mm')
+  then have sub1: "P \<turnstile> C1 \<prec>\<^sup>1 D"
+   by(auto simp: class_def fun_upd_apply intro!: subcls1I)
+  have cls: "\<And>D'. P \<turnstile> D \<preceq>\<^sup>* D' \<Longrightarrow> D' \<noteq> C"
+  proof -
+    fix D' assume "P \<turnstile> D \<preceq>\<^sup>* D'"
+    with sub1 have "P \<turnstile> C1 \<preceq>\<^sup>* D'" by simp
+    with rec.prems show "D' \<noteq> C" by simp
+  qed
+  with cls rec show ?case
+   by(auto simp: class_def fun_upd_apply intro: TypeRel.sees_methods_rec)
+qed
+
+lemma class_add_sees_methods_Obj:
+assumes "P \<turnstile> Object sees_methods Mm" and nObj: "C \<noteq> Object"
+shows "class_add P (C, cdec) \<turnstile> Object sees_methods Mm"
+proof -
+  from assms obtain C' fs ms where cls: "class P Object = Some(C',fs,ms)"
+     by(auto elim!: Methods.cases)
+  with nObj have cls': "class (class_add P (C, cdec)) Object = Some(C',fs,ms)"
+     by(simp add: class_def fun_upd_apply)
+  from assms cls have "Mm = map_option (\<lambda>m. (m, Object)) \<circ> map_of ms" by(auto elim!: Methods.cases)
+  with assms cls' show ?thesis
+   by(auto simp: is_class_def fun_upd_apply intro!: sees_methods_Object)
+qed
+
+lemma class_add_sees_methods_rev_Obj:
+assumes "class_add P (C, cdec) \<turnstile> Object sees_methods Mm" and nObj: "C \<noteq> Object"
+shows "P \<turnstile> Object sees_methods Mm"
+proof -
+  from assms obtain C' fs ms where cls: "class (class_add P (C, cdec)) Object = Some(C',fs,ms)"
+     by(auto elim!: Methods.cases)
+  with nObj have cls': "class P Object = Some(C',fs,ms)"
+     by(simp add: class_def fun_upd_apply)
+  from assms cls have "Mm = map_option (\<lambda>m. (m, Object)) \<circ> map_of ms" by(auto elim!: Methods.cases)
+  with assms cls' show ?thesis
+   by(auto simp: is_class_def fun_upd_apply intro!: sees_methods_Object)
+qed
+
+lemma class_add_sees_method:
+assumes "P \<turnstile> C\<^sub>0 sees M\<^sub>0, b : Ts\<rightarrow>T = m in D" and "\<not> is_class P C"
+shows "class_add P (C, cdec) \<turnstile> C\<^sub>0 sees M\<^sub>0, b : Ts\<rightarrow>T = m in D"
+using assms by(auto simp add: Method_def dest!: class_add_sees_methods[of P C\<^sub>0])
+
+lemma class_add_method:
+assumes md: "P \<turnstile> C\<^sub>0 sees M\<^sub>0, b : Ts\<rightarrow>T = m in D" and "\<not> is_class P C"
+shows "method P C\<^sub>0 M\<^sub>0 = method (class_add P (C, cdec)) C\<^sub>0 M\<^sub>0"
+using class_add_sees_method[OF assms, of cdec] md by simp
+
+lemma class_add_sees_method_rev:
+ "\<lbrakk> class_add P (C, cdec) \<turnstile> C\<^sub>0 sees M\<^sub>0, b : Ts\<rightarrow>T = m in D;
+    \<not> P \<turnstile> C\<^sub>0 \<preceq>\<^sup>* C \<rbrakk>
+  \<Longrightarrow> P \<turnstile> C\<^sub>0 sees M\<^sub>0, b : Ts\<rightarrow>T = m in D"
+ by(auto simp: Method_def dest!: class_add_sees_methods_rev)
+
+lemma class_add_sees_method_Obj:
+ "\<lbrakk> P \<turnstile> Object sees M\<^sub>0, b : Ts\<rightarrow>T = m in D; C \<noteq> Object \<rbrakk>
+  \<Longrightarrow> class_add P (C, cdec) \<turnstile> Object sees M\<^sub>0, b : Ts\<rightarrow>T = m in D"
+ by(auto simp add: Method_def dest!: class_add_sees_methods_Obj[where P=P])
+
+lemma class_add_sees_method_rev_Obj:
+ "\<lbrakk> class_add P (C, cdec) \<turnstile> Object sees M\<^sub>0, b : Ts\<rightarrow>T = m in D; C \<noteq> Object \<rbrakk>
+  \<Longrightarrow> P \<turnstile> Object sees M\<^sub>0, b : Ts\<rightarrow>T = m in D"
+ by(auto simp add: Method_def dest!: class_add_sees_methods_rev_Obj[where P=P])
+
+lemma class_add_is_type:
+ "is_type P T \<Longrightarrow> is_type (class_add P (C, cdec)) T"
+ by(cases cdec, simp add: is_type_def is_class_def class_def fun_upd_apply split: ty.splits)
+
+lemma class_add_types:
+ "types P \<subseteq> types (class_add P (C, cdec))"
+using class_add_is_type by(cases cdec, clarsimp)
+
+lemma class_add_states:
+ "states P mxs mxl \<subseteq> states (class_add P (C, cdec)) mxs mxl"
+proof -
+  let ?A = "types P" and ?B = "types (class_add P (C, cdec))"
+  have "?A \<subseteq> ?B" by(rule class_add_types)
+  then show ?thesis
+  apply(clarsimp simp: JVM_states_unfold intro!: err_mono opt_mono)
+  apply(unfold err_def list_def) apply(auto simp: Sigma_mono)
+  proof - (* ACTUALLY : make this proof better *)
+    fix a :: "ty list" and b :: "ty err list" and x :: "ty err"
+    assume a1: "x \<noteq> Err"
+    assume a2: "set b \<subseteq> insert Err {OK x |x. is_type P x}"
+    assume a3: "x \<in> set b"
+    assume a4: "types P \<subseteq> types (class_add P (C, cdec))"
+    have f5: "\<exists>t. x = OK t \<and> is_type P t" using a3 a2 a1 by blast
+    obtain tt :: "ty err \<Rightarrow> ty" where
+      f6: "((\<nexists>t. x = OK t \<and> is_type P t) \<or> x = OK (tt x) \<and> is_type P (tt x)) \<and> ((\<exists>t. x = OK t \<and> is_type P t) \<or> (\<forall>t. x \<noteq> OK t \<or> \<not> is_type P t))"
+      by moura
+    then have "tt x \<in> types P"
+      using f5 by blast
+    then have "is_type (class_add P (C, cdec)) (tt x)"
+      using a4 by blast
+    then show "\<exists>t. x = OK t \<and> is_type (class_add P (C, cdec)) t"
+      using f6 f5 by force
+  qed
+qed
+
+lemma class_add_check_types:
+ "check_types P mxs mxl \<tau>s \<Longrightarrow> check_types (class_add P (C, cdec)) mxs mxl \<tau>s"
+using class_add_states by(fastforce simp: check_types_def)
+
+lemma class_add_subcls:
+ "\<lbrakk> P \<turnstile> D \<preceq>\<^sup>* D'; \<not> is_class P C \<rbrakk>
+ \<Longrightarrow> class_add P (C, cdec) \<turnstile> D \<preceq>\<^sup>* D'"
+proof(induct rule: rtrancl.induct)
+  case (rtrancl_into_rtrancl a b c)
+  then have "b \<noteq> C" by(clarsimp simp: is_class_def dest!: subcls1D)
+  with rtrancl_into_rtrancl show ?case
+   by(fastforce dest!: subcls1D simp: class_def fun_upd_apply
+                intro!: rtrancl_trans[of a b] subcls1I)
+qed(simp)
+
+lemma class_add_subcls_rev:
+ "\<lbrakk> class_add P (C, cdec) \<turnstile> D \<preceq>\<^sup>* D'; \<not>P \<turnstile> D \<preceq>\<^sup>* C \<rbrakk>
+ \<Longrightarrow> P \<turnstile> D \<preceq>\<^sup>* D'"
+proof(induct rule: rtrancl.induct)
+  case (rtrancl_into_rtrancl a b c)
+  then have "b \<noteq> C" by(clarsimp simp: is_class_def dest!: subcls1D)
+  with rtrancl_into_rtrancl show ?case
+   by(fastforce dest!: subcls1D simp: class_def fun_upd_apply
+                intro!: rtrancl_trans[of a b] subcls1I)
+qed(simp)
+
+lemma class_add_subtype:
+ "\<lbrakk> subtype P x y; \<not> is_class P C \<rbrakk>
+ \<Longrightarrow> subtype (class_add P (C, cdec)) x y"
+proof(induct rule: widen.induct)
+  case (widen_subcls C D)
+  then show ?case using class_add_subcls by simp
+qed(simp+)
+
+lemma class_add_widens:
+ "\<lbrakk> P \<turnstile> Ts [\<le>] Ts'; \<not> is_class P C \<rbrakk>
+ \<Longrightarrow> (class_add P (C, cdec)) \<turnstile> Ts [\<le>] Ts'"
+using class_add_subtype by (metis (no_types) list_all2_mono)
+
+lemma class_add_sup_ty_opt:
+ "\<lbrakk> P \<turnstile> l1 \<le>\<^sub>\<top> l2; \<not> is_class P C \<rbrakk>
+  \<Longrightarrow> class_add P (C, cdec) \<turnstile> l1 \<le>\<^sub>\<top> l2"
+using class_add_subtype by(auto simp: sup_ty_opt_def Err.le_def lesub_def split: err.splits)
+
+lemma class_add_sup_loc:
+"\<lbrakk> P \<turnstile> LT [\<le>\<^sub>\<top>] LT'; \<not> is_class P C \<rbrakk>
+ \<Longrightarrow> class_add P (C, cdec) \<turnstile> LT [\<le>\<^sub>\<top>] LT'"
+using class_add_sup_ty_opt[where P=P and C=C] by (simp add: list.rel_mono_strong)
+
+lemma class_add_sup_state:
+ "\<lbrakk> P \<turnstile> \<tau> \<le>\<^sub>i \<tau>'; \<not> is_class P C \<rbrakk>
+  \<Longrightarrow> class_add P (C, cdec) \<turnstile> \<tau> \<le>\<^sub>i \<tau>'"
+using class_add_subtype class_add_sup_ty_opt
+ by(auto simp: sup_state_def Listn.le_def Product.le_def lesub_def class_add_widens
+               class_add_sup_ty_opt list_all2_mono)
+
+lemma class_add_sup_state_opt:
+ "\<lbrakk> P \<turnstile> \<tau> \<le>' \<tau>'; \<not> is_class P C \<rbrakk>
+ \<Longrightarrow> class_add P (C, cdec) \<turnstile> \<tau> \<le>' \<tau>'"
+ by(auto simp: sup_state_opt_def Opt.le_def lesub_def class_add_widens
+               class_add_sup_ty_opt list_all2_mono)
+
+lemma class_add_wf_mdecl:
+  "\<lbrakk> wf_mdecl wf_md P C\<^sub>0 md;
+     \<And>C\<^sub>0 md. wf_md P C\<^sub>0 md \<Longrightarrow> wf_md (class_add P (C, cdec)) C\<^sub>0 md \<rbrakk>
+  \<Longrightarrow> wf_mdecl wf_md (class_add P (C, cdec)) C\<^sub>0 md"
+ by(clarsimp simp: wf_mdecl_def class_add_is_type)
+
+lemma class_add_wf_mdecl':
+assumes wfd: "wf_mdecl wf_md P C\<^sub>0 md"
+  and ms: "(C\<^sub>0,S,fs,ms) \<in> set P" and md: "md \<in> set ms"
+  and wf_md': "\<And>C\<^sub>0 S fs ms m.\<lbrakk>(C\<^sub>0,S,fs,ms) \<in> set P; m \<in> set ms\<rbrakk> \<Longrightarrow> wf_md' (class_add P (C, cdec)) C\<^sub>0 m"
+shows "wf_mdecl wf_md' (class_add P (C, cdec)) C\<^sub>0 md"
+using assms by(clarsimp simp: wf_mdecl_def class_add_is_type)
+
+lemma class_add_wf_cdecl:
+assumes wfcd: "wf_cdecl wf_md P cd" and cdP: "cd \<in> set P"
+ and ncp: "\<not> P \<turnstile> fst cd \<preceq>\<^sup>* C" and dist: "distinct_fst P"
+ and wfmd: "\<And>C\<^sub>0 md. wf_md P C\<^sub>0 md \<Longrightarrow> wf_md (class_add P (C, cdec)) C\<^sub>0 md"
+ and nclass: "\<not> is_class P C"
+shows "wf_cdecl wf_md (class_add P (C, cdec)) cd"
+proof -
+  let ?P = "class_add P (C, cdec)"
+  obtain C1 D fs ms where [simp]: "cd = (C1,(D,fs,ms))" by(cases cd)
+  from wfcd
+  have "\<forall>f\<in>set fs. wf_fdecl ?P f" by(auto simp: wf_cdecl_def wf_fdecl_def class_add_is_type)
+  moreover
+  from wfcd wfmd class_add_wf_mdecl
+  have "\<forall>m\<in>set ms. wf_mdecl wf_md ?P C1 m" by(auto simp: wf_cdecl_def)
+  moreover
+  have "C1 \<noteq> Object \<Longrightarrow> is_class ?P D \<and> \<not> ?P \<turnstile> D \<preceq>\<^sup>* C1
+    \<and> (\<forall>(M,b,Ts,T,m)\<in>set ms.
+        \<forall>D' b' Ts' T' m'. ?P \<turnstile> D sees M,b':Ts' \<rightarrow> T' = m' in D' \<longrightarrow>
+                       b = b' \<and> ?P \<turnstile> Ts' [\<le>] Ts \<and> ?P \<turnstile> T \<le> T')"
+  proof -
+    assume nObj[simp]: "C1 \<noteq> Object"
+    with cdP dist have sub1: "P \<turnstile> C1 \<prec>\<^sup>1 D" by(auto simp: class_def intro!: subcls1I map_of_SomeI)
+    with ncp have ncp': "\<not> P \<turnstile> D \<preceq>\<^sup>* C" by(auto simp: converse_rtrancl_into_rtrancl)
+    with wfcd
+    have clsD: "is_class ?P D"
+     by(auto simp: wf_cdecl_def is_class_def class_def fun_upd_apply)
+    moreover
+    from wfcd sub1
+    have "\<not> ?P \<turnstile> D \<preceq>\<^sup>* C1" by(auto simp: wf_cdecl_def dest!: class_add_subcls_rev[OF _ ncp'])
+    moreover
+    have "\<And>M b Ts T m D' b' Ts' T' m'. (M,b,Ts,T,m) \<in> set ms
+            \<Longrightarrow> ?P \<turnstile> D sees M,b':Ts' \<rightarrow> T' = m' in D'
+            \<Longrightarrow> b = b' \<and> ?P \<turnstile> Ts' [\<le>] Ts \<and> ?P \<turnstile> T \<le> T'"
+    proof -
+      fix M b Ts T m D' b' Ts' T' m'
+      assume ms: "(M,b,Ts,T,m) \<in> set ms" and meth': "?P \<turnstile> D sees M,b':Ts' \<rightarrow> T' = m' in D'"
+      with sub1
+      have "P \<turnstile> D sees M,b':Ts' \<rightarrow> T' = m' in D'"
+       by(fastforce dest!: class_add_sees_method_rev[OF _ ncp'])
+      moreover
+      with wfcd ms meth'
+      have "b = b' \<and> P \<turnstile> Ts' [\<le>] Ts \<and> P \<turnstile> T \<le> T'"
+       by(cases m', fastforce simp: wf_cdecl_def elim!: ballE[where x="(M,b,Ts,T,m)"])
+      ultimately show "b = b' \<and> ?P \<turnstile> Ts' [\<le>] Ts \<and> ?P \<turnstile> T \<le> T'"
+       by(auto dest!: class_add_subtype[OF _ nclass] class_add_widens[OF _ nclass])
+    qed
+    ultimately show ?thesis by clarsimp
+  qed
+  moreover note wfcd
+  ultimately show ?thesis by(simp add: wf_cdecl_def)
+qed
+
+lemma class_add_wf_cdecl':
+assumes wfcd: "wf_cdecl wf_md P cd" and cdP: "cd \<in> set P"
+ and ncp: "\<not>P \<turnstile> fst cd \<preceq>\<^sup>* C" and dist: "distinct_fst P"
+ and wfmd: "\<And>C\<^sub>0 S fs ms m.\<lbrakk>(C\<^sub>0,S,fs,ms) \<in> set P; m \<in> set ms\<rbrakk> \<Longrightarrow> wf_md' (class_add P (C, cdec)) C\<^sub>0 m"
+ and nclass: "\<not> is_class P C"
+shows "wf_cdecl wf_md' (class_add P (C, cdec)) cd"
+proof -
+  let ?P = "class_add P (C, cdec)"
+  obtain C1 D fs ms where [simp]: "cd = (C1,(D,fs,ms))" by(cases cd)
+  from wfcd
+  have "\<forall>f\<in>set fs. wf_fdecl ?P f" by(auto simp: wf_cdecl_def wf_fdecl_def class_add_is_type)
+  moreover
+  from cdP wfcd wfmd
+  have "\<forall>m\<in>set ms. wf_mdecl wf_md' ?P C1 m"
+    by(auto simp: wf_cdecl_def wf_mdecl_def class_add_is_type)
+  moreover
+  have "C1 \<noteq> Object \<Longrightarrow> is_class ?P D \<and> \<not> ?P \<turnstile> D \<preceq>\<^sup>* C1
+    \<and> (\<forall>(M,b,Ts,T,m)\<in>set ms.
+        \<forall>D' b' Ts' T' m'. ?P \<turnstile> D sees M,b':Ts' \<rightarrow> T' = m' in D' \<longrightarrow>
+                       b = b' \<and> ?P \<turnstile> Ts' [\<le>] Ts \<and> ?P \<turnstile> T \<le> T')"
+  proof -
+    assume nObj[simp]: "C1 \<noteq> Object"
+    with cdP dist have sub1: "P \<turnstile> C1 \<prec>\<^sup>1 D" by(auto simp: class_def intro!: subcls1I map_of_SomeI)
+    with ncp have ncp': "\<not> P \<turnstile> D \<preceq>\<^sup>* C" by(auto simp: converse_rtrancl_into_rtrancl)
+    with wfcd
+    have clsD: "is_class ?P D"
+     by(auto simp: wf_cdecl_def is_class_def class_def fun_upd_apply)
+    moreover
+    from wfcd sub1
+    have "\<not> ?P \<turnstile> D \<preceq>\<^sup>* C1" by(auto simp: wf_cdecl_def dest!: class_add_subcls_rev[OF _ ncp'])
+    moreover
+    have "\<And>M b Ts T m D' b' Ts' T' m'. (M,b,Ts,T,m) \<in> set ms
+            \<Longrightarrow> ?P \<turnstile> D sees M,b':Ts' \<rightarrow> T' = m' in D'
+            \<Longrightarrow> b = b' \<and> ?P \<turnstile> Ts' [\<le>] Ts \<and> ?P \<turnstile> T \<le> T'"
+    proof -
+      fix M b Ts T m D' b' Ts' T' m'
+      assume ms: "(M,b,Ts,T,m) \<in> set ms" and meth': "?P \<turnstile> D sees M,b':Ts' \<rightarrow> T' = m' in D'"
+      with sub1
+      have "P \<turnstile> D sees M,b':Ts' \<rightarrow> T' = m' in D'"
+       by(fastforce dest!: class_add_sees_method_rev[OF _ ncp'])
+      moreover
+      with wfcd ms meth'
+      have "b = b' \<and> P \<turnstile> Ts' [\<le>] Ts \<and> P \<turnstile> T \<le> T'"
+       by(cases m', fastforce simp: wf_cdecl_def elim!: ballE[where x="(M,b,Ts,T,m)"])
+      ultimately show "b = b' \<and> ?P \<turnstile> Ts' [\<le>] Ts \<and> ?P \<turnstile> T \<le> T'"
+       by(auto dest!: class_add_subtype[OF _ nclass] class_add_widens[OF _ nclass])
+    qed
+    ultimately show ?thesis by clarsimp
+  qed
+  moreover note wfcd
+  ultimately show ?thesis by(simp add: wf_cdecl_def)
+qed
+
+lemma class_add_app\<^sub>i:
+assumes "app\<^sub>i (i, P, pc, mxs, T\<^sub>r, ST, LT)" and "\<not> is_class P C"
+shows "app\<^sub>i (i, class_add P (C, cdec), pc, mxs, T\<^sub>r, ST, LT)"
+using assms
+proof(cases i)
+  case New then show ?thesis using assms by(fastforce simp: is_class_def class_def fun_upd_apply)
+next
+  case Getfield then show ?thesis using assms
+   by(auto simp: class_add_subtype dest!: class_add_sees_field[where P=P])
+next
+  case Getstatic then show ?thesis using assms by(auto dest!: class_add_sees_field[where P=P])
+next
+  case Putfield then show ?thesis using assms
+   by(auto dest!: class_add_subtype[where P=P] class_add_sees_field[where P=P])
+next
+  case Putstatic then show ?thesis using assms
+   by(auto dest!: class_add_subtype[where P=P] class_add_sees_field[where P=P])
+next
+  case Checkcast then show ?thesis using assms
+   by(clarsimp simp: is_class_def class_def fun_upd_apply)
+next
+  case Invoke then show ?thesis using assms
+    by(fastforce dest!: class_add_widens[where P=P] class_add_sees_method[where P=P])
+next
+  case Invokestatic then show ?thesis using assms
+    by(fastforce dest!: class_add_widens[where P=P] class_add_sees_method[where P=P])
+next
+  case Return then show ?thesis using assms by(clarsimp simp: class_add_subtype)
+qed(simp+)
+
+lemma class_add_wt_start:
+ "\<lbrakk> wt_start P C\<^sub>0 b Ts mxl \<tau>s; \<not> is_class P C \<rbrakk>
+ \<Longrightarrow> wt_start (class_add P (C, cdec)) C\<^sub>0 b Ts mxl \<tau>s"
+using class_add_sup_state_opt by(clarsimp simp: wt_start_def split: staticb.splits)
+
+lemma class_add_is_relevant_class:
+ "\<lbrakk> is_relevant_class i P C\<^sub>0; \<not> is_class P C \<rbrakk>
+  \<Longrightarrow> is_relevant_class i (class_add P (C, cdec)) C\<^sub>0"
+  by(cases i, auto simp: class_add_subcls)
+
+lemma class_add_is_relevant_class_rev:
+assumes irc: "is_relevant_class i (class_add P (C, cdec)) C\<^sub>0"
+  and ncp: "\<And>cd D'. cd \<in> set P \<Longrightarrow> \<not>P \<turnstile> fst cd \<preceq>\<^sup>* C"
+  and wfxp: "wf_syscls P"
+shows "is_relevant_class i P C\<^sub>0"
+using assms
+proof(cases i)
+  case (Getfield F D) with assms
+  show ?thesis by(fastforce simp: wf_syscls_def sys_xcpts_def dest!: class_add_subcls_rev)
+next
+  case (Putfield F D) with assms
+  show ?thesis by(fastforce simp: wf_syscls_def sys_xcpts_def dest!: class_add_subcls_rev)
+next
+  case (Checkcast D) with assms
+  show ?thesis by(fastforce simp: wf_syscls_def sys_xcpts_def dest!: class_add_subcls_rev)
+qed(simp_all)
+
+lemma class_add_is_relevant_entry:
+ "\<lbrakk> is_relevant_entry P i pc e; \<not> is_class P C \<rbrakk>
+  \<Longrightarrow> is_relevant_entry (class_add P (C, cdec)) i pc e"
+ by(clarsimp simp: is_relevant_entry_def class_add_is_relevant_class)
+
+lemma class_add_is_relevant_entry_rev:
+ "\<lbrakk> is_relevant_entry (class_add P (C, cdec)) i pc e; 
+    \<And>cd D'. cd \<in> set P \<Longrightarrow> \<not>P \<turnstile> fst cd \<preceq>\<^sup>* C;
+    wf_syscls P \<rbrakk>
+  \<Longrightarrow> is_relevant_entry P i pc e"
+ by(auto simp: is_relevant_entry_def dest!: class_add_is_relevant_class_rev)
+
+lemma class_add_relevant_entries:
+ "\<not> is_class P C
+  \<Longrightarrow> set (relevant_entries P i pc xt) \<subseteq> set (relevant_entries (class_add P (C, cdec)) i pc xt)"
+ by(clarsimp simp: relevant_entries_def class_add_is_relevant_entry)
+
+lemma class_add_relevant_entries_eq:
+assumes wf: "wf_prog wf_md P" and nclass: "\<not> is_class P C"
+shows "relevant_entries P i pc xt = relevant_entries (class_add P (C, cdec)) i pc xt"
+proof -
+  have ncp: "\<And>cd D'. cd \<in> set P \<Longrightarrow> \<not>P \<turnstile> fst cd \<preceq>\<^sup>* C"
+   by(rule wf_subcls_nCls'[OF assms])
+  moreover from wf have wfsys: "wf_syscls P" by(simp add: wf_prog_def)
+  moreover
+  note class_add_is_relevant_entry[OF _ nclass, of i pc _ cdec]
+       class_add_is_relevant_entry_rev[OF _ ncp wfsys, of cdec i pc]
+  ultimately show ?thesis by (metis filter_cong relevant_entries_def)
+qed
+
+lemma class_add_xcpt_app:
+assumes xa: "xcpt_app i P pc mxs xt \<tau>"
+ and wf: "wf_prog wf_md P" and nclass: "\<not> is_class P C"
+shows "xcpt_app i (class_add P (C, cdec)) pc mxs xt \<tau>"
+using xa class_add_relevant_entries_eq[OF wf nclass] nclass
+ by(auto simp: xcpt_app_def is_class_def class_def fun_upd_apply) auto
+
+lemma class_add_norm_eff_pc:
+assumes ne: "\<forall>(pc',\<tau>') \<in> set (norm_eff i P pc \<tau>). pc' < mpc"
+shows "\<forall>(pc',\<tau>') \<in> set (norm_eff i (class_add P (C, cdec)) pc \<tau>). pc' < mpc"
+using assms by(cases i, auto simp: norm_eff_def)
+
+lemma class_add_norm_eff_sup_state_opt:
+assumes ne: "\<forall>(pc',\<tau>') \<in> set (norm_eff i P pc \<tau>). P \<turnstile> \<tau>' \<le>' \<tau>s!pc'"
+   and nclass: "\<not> is_class P C" and app: "app\<^sub>i (i, P, pc, mxs, T, \<tau>)"
+shows "\<forall>(pc',\<tau>') \<in> set (norm_eff i (class_add P (C, cdec)) pc \<tau>). (class_add P (C, cdec)) \<turnstile> \<tau>' \<le>' \<tau>s!pc'"
+proof -
+  obtain ST LT where "\<tau> = (ST,LT)" by(cases \<tau>)
+  with assms show ?thesis proof(cases i)
+  qed(fastforce simp: norm_eff_def
+                dest!: class_add_field[where cdec=cdec] class_add_method[where cdec=cdec]
+                       class_add_sup_loc[OF _ nclass] class_add_subtype[OF _ nclass]
+                       class_add_widens[OF _ nclass] class_add_sup_state_opt[OF _ nclass])+
+qed
+
+lemma class_add_xcpt_eff_eq:
+assumes wf: "wf_prog wf_md P" and nclass: "\<not> is_class P C"
+shows "xcpt_eff i P pc \<tau> xt = xcpt_eff i (class_add P (C, cdec)) pc \<tau> xt"
+using class_add_relevant_entries_eq[OF assms, of i pc xt cdec] by(cases \<tau>, simp add: xcpt_eff_def)
+
+lemma class_add_eff_pc:
+assumes eff: "\<forall>(pc',\<tau>') \<in> set (eff i P pc xt (Some \<tau>)). pc' < mpc"
+  and wf: "wf_prog wf_md P" and nclass: "\<not> is_class P C"
+shows "\<forall>(pc',\<tau>') \<in> set (eff i (class_add P (C, cdec)) pc xt (Some \<tau>)). pc' < mpc"
+using eff class_add_norm_eff_pc class_add_xcpt_eff_eq[OF wf nclass]
+  by(auto simp: norm_eff_def eff_def)
+
+lemma class_add_eff_sup_state_opt:
+assumes eff: "\<forall>(pc',\<tau>') \<in> set (eff i P pc xt (Some \<tau>)). P \<turnstile> \<tau>' \<le>' \<tau>s!pc'"
+  and wf: "wf_prog wf_md P"and nclass: "\<not> is_class P C"
+  and app: "app\<^sub>i (i, P, pc, mxs, T, \<tau>)"
+shows "\<forall>(pc',\<tau>') \<in> set (eff i (class_add P (C, cdec)) pc xt (Some \<tau>)).
+         (class_add P (C, cdec)) \<turnstile> \<tau>' \<le>' \<tau>s!pc'"
+proof -
+  from eff have ne: "\<forall>(pc', \<tau>')\<in>set (norm_eff i P pc \<tau>). P \<turnstile> \<tau>' \<le>' \<tau>s ! pc'"
+   by(simp add: norm_eff_def eff_def)
+  from eff have "\<forall>(pc', \<tau>')\<in>set (xcpt_eff i P pc \<tau> xt). P \<turnstile> \<tau>' \<le>' \<tau>s ! pc'"
+   by(simp add: xcpt_eff_def eff_def)
+  with class_add_norm_eff_sup_state_opt[OF ne nclass app]
+       class_add_xcpt_eff_eq[OF wf nclass]class_add_sup_state_opt[OF _ nclass]
+    show ?thesis by(cases cdec, auto simp: eff_def norm_eff_def xcpt_app_def)
+qed
+
+lemma class_add_app:
+assumes app: "app i P mxs T pc mpc xt t"
+ and wf: "wf_prog wf_md P" and nclass: "\<not> is_class P C"
+shows "app i (class_add P (C, cdec)) mxs T pc mpc xt t"
+proof(cases t)
+  case (Some \<tau>)
+  let ?P = "class_add P (C, cdec)"
+  from assms Some have eff: "\<forall>(pc', \<tau>')\<in>set (eff i P pc xt \<lfloor>\<tau>\<rfloor>). pc' < mpc" by(simp add: app_def)
+  from assms Some have app\<^sub>i: "app\<^sub>i (i,P,pc,mxs,T,\<tau>)" by(simp add: app_def)
+  with class_add_app\<^sub>i[OF _ nclass] Some have "app\<^sub>i (i,?P,pc,mxs,T,\<tau>)" by(cases \<tau>,simp)
+  moreover
+  from app class_add_xcpt_app[OF _ wf nclass] Some
+  have "xcpt_app i ?P pc mxs xt \<tau>" by(simp add: app_def del: xcpt_app_def)
+  moreover
+  from app class_add_eff_pc[OF eff wf nclass] Some
+  have "\<forall>(pc',\<tau>') \<in> set (eff i ?P pc xt t). pc' < mpc" by auto
+  moreover note app Some
+  ultimately show ?thesis by(simp add: app_def)
+qed(simp)
+
+lemma class_add_wt_instr:
+assumes wti: "P,T,mxs,mpc,xt \<turnstile> i,pc :: \<tau>s"
+ and wf: "wf_prog wf_md P" and nclass: "\<not> is_class P C"
+shows "class_add P (C, cdec),T,mxs,mpc,xt \<turnstile> i,pc :: \<tau>s"
+proof -
+  let ?P = "class_add P (C, cdec)"
+  from wti have eff: "\<forall>(pc', \<tau>')\<in>set (eff i P pc xt (\<tau>s ! pc)). P \<turnstile> \<tau>' \<le>' \<tau>s ! pc'"
+   by(simp add: wt_instr_def)
+  from wti have app\<^sub>i: "\<tau>s!pc \<noteq> None \<Longrightarrow> app\<^sub>i (i,P,pc,mxs,T,the (\<tau>s!pc))"
+   by(simp add: wt_instr_def app_def)
+  from wti class_add_app[OF _ wf nclass]
+  have "app i ?P mxs T pc mpc xt (\<tau>s!pc)" by(simp add: wt_instr_def)
+  moreover
+  have "\<forall>(pc',\<tau>') \<in> set (eff i ?P pc xt (\<tau>s!pc)). ?P \<turnstile> \<tau>' \<le>' \<tau>s!pc'"
+  proof(cases "\<tau>s!pc")
+    case Some with eff class_add_eff_sup_state_opt[OF _ wf nclass app\<^sub>i] show ?thesis by auto
+  qed(simp add: eff_def)
+  moreover note wti
+  ultimately show ?thesis by(clarsimp simp: wt_instr_def)
+qed
+
+lemma class_add_wt_method:
+assumes wtm: "wt_method P C\<^sub>0 b Ts T\<^sub>r mxs mxl\<^sub>0 is xt (\<Phi> C\<^sub>0 M\<^sub>0)"
+ and wf: "wf_prog wf_md P" and nclass: "\<not> is_class P C"
+shows "wt_method (class_add P (C, cdec)) C\<^sub>0 b Ts T\<^sub>r mxs mxl\<^sub>0 is xt (\<Phi> C\<^sub>0 M\<^sub>0)"
+proof -
+  let ?P = "class_add P (C, cdec)"
+  let ?\<tau>s = "\<Phi> C\<^sub>0 M\<^sub>0"
+  from wtm class_add_check_types
+  have "check_types ?P mxs ((case b of Static \<Rightarrow> 0 | NonStatic \<Rightarrow> 1)+size Ts+mxl\<^sub>0) (map OK ?\<tau>s)"
+   by(simp add: wt_method_def)
+  moreover
+  from wtm class_add_wt_start nclass
+  have "wt_start ?P C\<^sub>0 b Ts mxl\<^sub>0 ?\<tau>s" by(simp add: wt_method_def)
+  moreover
+  from wtm class_add_wt_instr[OF _ wf nclass]
+  have "\<forall>pc < size is. ?P,T\<^sub>r,mxs,size is,xt \<turnstile> is!pc,pc :: ?\<tau>s" by(clarsimp simp: wt_method_def)
+  moreover note wtm
+  ultimately
+  show ?thesis by(clarsimp simp: wt_method_def)
+qed
+
+lemma class_add_wt_method':
+ "\<lbrakk> (\<lambda>P C (M,b,Ts,T\<^sub>r,(mxs,mxl\<^sub>0,is,xt)). wt_method P C b Ts T\<^sub>r mxs mxl\<^sub>0 is xt (\<Phi> C M)) P C\<^sub>0 md;
+    wf_prog wf_md P; \<not> is_class P C \<rbrakk>
+    \<Longrightarrow> (\<lambda>P C (M,b,Ts,T\<^sub>r,(mxs,mxl\<^sub>0,is,xt)). wt_method P C b Ts T\<^sub>r mxs mxl\<^sub>0 is xt (\<Phi> C M))
+            (class_add P (C, cdec)) C\<^sub>0 md"
+ by(clarsimp simp: class_add_wt_method)
+
+lemma class_add_distinct_fst:
+"\<lbrakk> distinct_fst P; \<not> is_class P C \<rbrakk>
+  \<Longrightarrow> distinct_fst (class_add P (C, cdec))"
+ by(clarsimp simp add: distinct_fst_def is_class_def class_def)
+
+(**********************************************)
+
+(* HERE: MOVE *)
+lemma class_add_classes_above:
+assumes ns: "\<not> is_class P C" and "\<not>P \<turnstile> D \<preceq>\<^sup>* C"
+shows "classes_above (class_add P (C, cdec)) D = classes_above P D"
+using assms by(auto intro: class_add_subcls class_add_subcls_rev)
+
+(* HERE: MOVE *)
+lemma class_add_classes_above_xcpts:
+assumes ns: "\<not> is_class P C"
+ and ncp: "\<And>D. D \<in> sys_xcpts \<Longrightarrow> \<not>P \<turnstile> D \<preceq>\<^sup>* C"
+shows "classes_above_xcpts (class_add P (C, cdec)) = classes_above_xcpts P"
+using assms class_add_classes_above by simp
+
+(*****************************************************************************)
+
+(***)
+
+(* HERE: MOVE ! ! *)
+lemma class_add_conf:
+ "\<lbrakk> P,h \<turnstile> v :\<le> T; \<not> is_class P C \<rbrakk>
+ \<Longrightarrow> class_add P (C, cdec),h \<turnstile> v :\<le> T"
+ by(clarsimp simp: conf_def class_add_subtype)
+
+(* HERE: MOVE ! ! -- will not need fixes if above correct_state def *)
+lemma class_add_oconf:
+fixes obj::obj
+assumes oc: "P,h \<turnstile> obj \<surd>" and ns: "\<not> is_class P C"
+  and ncp: "\<And>D'. P \<turnstile> fst(obj) \<preceq>\<^sup>* D' \<Longrightarrow> D' \<noteq> C"
+shows "(class_add P (C, cdec)),h \<turnstile> obj \<surd>"
+proof -
+  obtain C\<^sub>0 fs where [simp]: "obj=(C\<^sub>0,fs)" by(cases obj)
+  from oc have
+    oc': "\<And>F D T. P \<turnstile> C\<^sub>0 has F,NonStatic:T in D \<Longrightarrow> (\<exists>v. fs (F, D) = \<lfloor>v\<rfloor> \<and> P,h \<turnstile> v :\<le> T)"
+    by(simp add: oconf_def)
+  have "\<And>F D T. class_add P (C, cdec) \<turnstile> C\<^sub>0 has F,NonStatic:T in D
+                       \<Longrightarrow> \<exists>v. fs(F,D) = Some v \<and> class_add P (C, cdec),h \<turnstile> v :\<le> T"
+  proof -
+    fix F D T assume "class_add P (C, cdec) \<turnstile> C\<^sub>0 has F,NonStatic:T in D"
+    with class_add_has_field_rev[OF _ ncp] have meth: "P \<turnstile> C\<^sub>0 has F,NonStatic:T in D" by simp
+    then show "\<exists>v. fs(F,D) = Some v \<and> class_add P (C, cdec),h \<turnstile> v :\<le> T"
+    using oc'[OF meth] class_add_conf[OF _ ns] by(fastforce simp: oconf_def)
+  qed
+  then show ?thesis by(simp add: oconf_def)
+qed
+
+(* HERE: MOVE ! ! *)
+lemma class_add_soconf:
+assumes soc: "P,h,C\<^sub>0 \<turnstile>\<^sub>s sfs \<surd>" and ns: "\<not> is_class P C"
+  and ncp: "\<And>D'. P \<turnstile> C\<^sub>0 \<preceq>\<^sup>* D' \<Longrightarrow> D' \<noteq> C"
+shows "(class_add P (C, cdec)),h,C\<^sub>0 \<turnstile>\<^sub>s sfs \<surd>"
+proof -
+  from soc have
+    oc': "\<And>F T. P \<turnstile> C\<^sub>0 has F,Static:T in C\<^sub>0 \<Longrightarrow> (\<exists>v. sfs F = \<lfloor>v\<rfloor> \<and> P,h \<turnstile> v :\<le> T)"
+    by(simp add: soconf_def)
+  have "\<And>F T. class_add P (C, cdec) \<turnstile> C\<^sub>0 has F,Static:T in C\<^sub>0
+                       \<Longrightarrow> \<exists>v. sfs F = Some v \<and> class_add P (C, cdec),h \<turnstile> v :\<le> T"
+  proof -
+    fix F T assume "class_add P (C, cdec) \<turnstile> C\<^sub>0 has F,Static:T in C\<^sub>0"
+    with class_add_has_field_rev[OF _ ncp] have meth: "P \<turnstile> C\<^sub>0 has F,Static:T in C\<^sub>0" by simp
+    then show "\<exists>v. sfs F = Some v \<and> class_add P (C, cdec),h \<turnstile> v :\<le> T"
+    using oc'[OF meth] class_add_conf[OF _ ns] by(fastforce simp: soconf_def)
+  qed
+  then show ?thesis by(simp add: soconf_def)
+qed
+
+lemma class_add_hconf:
+assumes "P \<turnstile> h \<surd>" and "\<not> is_class P C"
+ and "\<And>a obj D'. h a = Some obj \<Longrightarrow> P \<turnstile> fst(obj) \<preceq>\<^sup>* D' \<Longrightarrow> D' \<noteq> C"
+shows "class_add P (C, cdec) \<turnstile> h \<surd>"
+using assms by(auto simp: hconf_def intro!: class_add_oconf)
+
+lemma class_add_hconf_wf:
+assumes wf: "wf_prog wf_md P" and "P \<turnstile> h \<surd>" and "\<not> is_class P C"
+ and "\<And>a obj. h a = Some obj \<Longrightarrow> fst(obj) \<noteq> C"
+shows "class_add P (C, cdec) \<turnstile> h \<surd>"
+using wf_subcls_nCls[OF wf] assms by(fastforce simp: hconf_def intro!: class_add_oconf)
+
+lemma class_add_shconf:
+assumes "P,h \<turnstile>\<^sub>s sh \<surd>" and ns: "\<not> is_class P C"
+ and "\<And>C sobj D'. sh C = Some sobj \<Longrightarrow> P \<turnstile> C \<preceq>\<^sup>* D' \<Longrightarrow> D' \<noteq> C"
+shows "class_add P (C, cdec),h \<turnstile>\<^sub>s sh \<surd>"
+using assms by(fastforce simp: shconf_def)
+
+lemma class_add_shconf_wf:
+assumes wf: "wf_prog wf_md P" and "P,h \<turnstile>\<^sub>s sh \<surd>" and "\<not> is_class P C"
+ and "\<And>C sobj. sh C = Some sobj \<Longrightarrow> C \<noteq> C"
+shows "class_add P (C, cdec),h \<turnstile>\<^sub>s sh \<surd>"
+using wf_subcls_nCls[OF wf] assms by(fastforce simp add: shconf_def)
+
+(******************************************)
+
+(* ACTUALLY: generalize
+lemma class_add_wf_jvm_prog_phi:
+assumes wtp: "wf_jvm_prog\<^bsub>\<Phi>\<^esub> P"
+ and nclass: "\<not> is_class P C"
+ and meth: "P \<turnstile> C sees M, Static :  []\<rightarrow>Void = m in D" and nclinit: "M \<noteq> clinit"
+ and \<Phi>: "\<And>C'. C' \<noteq> C \<Longrightarrow> \<Phi>' C' = \<Phi> C'"
+ and \<Phi>': "\<Phi>' C start_m = start_\<phi>\<^sub>m" "\<Phi>' C clinit = start_\<phi>\<^sub>m"
+ and Obj_start_m: "\<And>b' Ts' T' m' D'. P \<turnstile> Object sees start_m, b' :  Ts'\<rightarrow>T' = m' in D'
+         \<Longrightarrow> b' = Static \<and> Ts' = [] \<and> T' = Void"
+shows "wf_jvm_prog\<^bsub>\<Phi>'\<^esub> (class_add P (C, cdec))"
+proof -
+  let ?wf_md = "(\<lambda>P C (M,b,Ts,T\<^sub>r,(mxs,mxl\<^sub>0,is,xt)). wt_method P C b Ts T\<^sub>r mxs mxl\<^sub>0 is xt (\<Phi> C M))"
+  let ?wf_md' = "(\<lambda>P C (M,b,Ts,T\<^sub>r,(mxs,mxl\<^sub>0,is,xt)). wt_method P C b Ts T\<^sub>r mxs mxl\<^sub>0 is xt (\<Phi>' C M))"
+  from wtp have wf: "wf_prog ?wf_md P" by(simp add: wf_jvm_prog_phi_def)
+  from wf_subcls_nCls'[OF wf nclass]
+  have ncp: "\<And>cd D'. cd \<in> set P \<Longrightarrow> \<not>P \<turnstile> fst cd \<preceq>\<^sup>* C" by simp
+  have wf_md':
+    "\<And>C\<^sub>0 S fs ms m. (C\<^sub>0, S, fs, ms) \<in> set P \<Longrightarrow> m \<in> set ms \<Longrightarrow> ?wf_md' (class_add P (C, cdec)) C\<^sub>0 m"
+  proof -
+    fix C\<^sub>0 S fs ms m assume asms: "(C\<^sub>0, S, fs, ms) \<in> set P" "m \<in> set ms"
+    with nclass have ns: "C\<^sub>0 \<noteq> C" by(auto simp: is_class_def class_def dest: weak_map_of_SomeI)
+    from wf asms have "?wf_md P C\<^sub>0 m" by(auto simp: wf_prog_def wf_cdecl_def wf_mdecl_def)
+
+    with \<Phi>[OF ns] class_add_wt_method[OF _ wf nclass]
+     show "?wf_md' (class_add P (C, cdec)) C\<^sub>0 m" by fastforce
+  qed
+  from wtp have a1: "is_class P Object" by (simp add: wf_jvm_prog_phi_def)
+  with wf_sees_clinit[where P=P and C=Object] wtp
+   have a2: "\<And>b' Ts' T' m' D'. P \<turnstile> Object sees clinit, b' :  Ts'\<rightarrow>T' = m' in D'
+         \<Longrightarrow> b' = Static \<and> Ts' = [] \<and> T' = Void"
+    by(fastforce simp: wf_jvm_prog_phi_def is_class_def dest: sees_method_fun)
+  from wf have dist: "distinct_fst P" by (simp add: wf_prog_def)
+  then have "distinct_fst (class_add P (C, cdec))" by(rule class_add_distinct_fst[OF _ nclass])
+  moreover from wf have "wf_syscls (class_add P (C, cdec))" by(simp add: wf_prog_def wf_syscls_def)
+  moreover
+  from class_add_wf_cdecl'[where wf_md'="?wf_md'", OF _ _ ncp dist wf_md' nclass] wf
+  have "\<And>c. c \<in> set P \<Longrightarrow> wf_cdecl ?wf_md' (class_add P (C, cdec)) c" by(auto simp: wf_prog_def)
+  moreover from meth nclinit nclass \<Phi>' a1 Obj_start_m a2
+  have "wf_cdecl ?wf_md' (class_add P (C, cdec)) (start_class C M)" by(simp add: start_class_wf)
+  ultimately show ?thesis by(simp add: wf_jvm_prog_phi_def wf_prog_def)
+qed
+
+lemma class_add_wf_jvm_prog:
+assumes wf: "wf_jvm_prog P"
+ and nclass: "\<not> is_class P C"
+ and meth: "P \<turnstile> C sees M, Static :  []\<rightarrow>Void = m in D" and nclinit: "M \<noteq> clinit"
+ and Obj_start_m: "\<And>b' Ts' T' m' D'. P \<turnstile> Object sees start_m, b' :  Ts'\<rightarrow>T' = m' in D'
+         \<Longrightarrow> b' = Static \<and> Ts' = [] \<and> T' = Void"
+shows "wf_jvm_prog (class_add P (C, cdec))"
+proof -
+  from wf obtain \<Phi> where wtp: "wf_jvm_prog\<^bsub>\<Phi>\<^esub> P" by(clarsimp simp: wf_jvm_prog_def)
+
+  let ?\<Phi>' = "\<lambda>C f. if C = C \<and> (f = start_m \<or> f = clinit) then start_\<phi>\<^sub>m else \<Phi> C f"
+
+  from class_add_wf_jvm_prog_phi[OF wtp nclass meth nclinit _ _ _ Obj_start_m] have
+    "wf_jvm_prog\<^bsub>?\<Phi>'\<^esub> (class_add P (C, cdec))" by simp
+  then show ?thesis by(auto simp: wf_jvm_prog_def)
+qed
+
+
+lemma class_add_Start_sees_methods:
+ "P \<turnstile> Object sees_methods Mm
+ \<Longrightarrow> class_add P (C, cdec) \<turnstile>
+  C sees_methods Mm ++ (map_option (\<lambda>m. (m,Start)) \<circ> map_of [start_method C M, start_clinit])"
+ by (auto simp: start_class_def class_def fun_upd_apply
+          dest!: class_add_sees_methods_Obj[of P] intro: sees_methods_rec)
+
+lemma class_add_Start_sees_start_method:
+ "P \<turnstile> Object sees_methods Mm
+  \<Longrightarrow> class_add P (C, cdec) \<turnstile>
+         C sees start_m, Static : []\<rightarrow>Void = (1, 0, [Invokestatic C M 0,Return], []) in C"
+ by(auto simp: start_class_def start_method_def Method_def fun_upd_apply
+         dest!: class_add_Start_sees_methods)
+
+(* HERE: MOVE *)
+lemma wf_class_add_Start_sees_start_method:
+assumes wf: "wf_prog wf_md P"
+shows "class_add P (C, cdec) \<turnstile>
+         C sees start_m, Static : []\<rightarrow>Void = (1, 0, [Invokestatic C M 0,Return], []) in C"
+proof -
+  from wf have "is_class P Object" by simp
+  with sees_methods_Object  obtain Mm where "P \<turnstile> Object sees_methods Mm"
+   by(fastforce simp: is_class_def dest: sees_methods_Object)
+  then show ?thesis by(rule class_add_Start_sees_start_method)
+qed
+
+(* HERE: MOVE *)
+lemma class_add_start_m_instrs:
+assumes wf: "wf_prog wf_md P"
+shows "(instrs_of (class_add P (C, cdec)) C start_m) = [Invokestatic C M 0, Return]"
+proof -
+  from wf_class_add_Start_sees_start_method[OF wf]
+  have "class_add P (C, cdec) \<turnstile> C sees start_m, Static :
+           []\<rightarrow>Void = (1,0,[Invokestatic C M 0,Return],[]) in C" by simp
+  then show ?thesis by simp
+qed
+
+
+(* HERE: MOVE ? *)
+lemma class_add_Start_fields:
+ "class_add P (C, cdec) \<turnstile> C has_fields FDTs \<Longrightarrow> map_of FDTs (F, C) = None"
+ by(drule Fields.cases, auto simp: start_class_def class_def fun_upd_apply Object_fields)
+
+lemma class_add_Start_soconf:
+ "(class_add P (C, cdec)),h,Start \<turnstile>\<^sub>s Map.empty \<surd>"
+ by(simp add: soconf_def has_field_def class_add_Start_fields)
+
+lemma class_add_start_shconf:
+ "class_add P (C, cdec),start_heap P \<turnstile>\<^sub>s start_sheap \<surd>"
+(*<*)
+  apply (unfold shconf_def)
+  apply (simp add: preallocated_start fun_upd_apply class_add_Start_soconf)
+  done
+(*>*)
+*)
+
+(*************************************)
+
+end
