Common/ClassesBetween.thy
@@ -1,0 +1,625 @@
+(*  Title:      Jinja/Common/ClassesBetween.thy
+    Author:    Susannah Mansky, UIUC 2016
+*)
+
+section {* Theory around the classes between two class in the class structure,
+ in particular noting that if they have not changed, then what the
+ subclass sees (methods, fields) found between the two stays the same. *}
+
+theory ClassesBetween
+imports ClassesChanged MethodsAndFields
+begin
+
+
+lemma classes_between_subset_below:
+ "\<lbrakk> P \<turnstile> C \<preceq>\<^sup>* C'; P \<turnstile> C' \<preceq>\<^sup>* C'' \<rbrakk>
+ \<Longrightarrow> classes_between P C C' \<subseteq> classes_between P C C''"
+ by auto
+
+lemma classes_between_subset_above:
+ "\<lbrakk> P \<turnstile> C \<preceq>\<^sup>* C'; P \<turnstile> C' \<preceq>\<^sup>* C'' \<rbrakk>
+ \<Longrightarrow> classes_between P C' C'' \<subseteq> classes_between P C C''"
+ by auto
+
+lemma classes_between_subset_between:
+ "\<lbrakk> P \<turnstile> C \<preceq>\<^sup>* C'; P \<turnstile> C' \<preceq>\<^sup>* C''; P \<turnstile> C'' \<preceq>\<^sup>* C''' \<rbrakk>
+ \<Longrightarrow> classes_between P C' C'' \<subseteq> classes_between P C C'''"
+ by auto
+
+
+(**)
+
+lemma classes_between_unchanged:
+ "\<lbrakk> classes_between P C C' \<inter> classes_changed P P' = {}; P \<turnstile> C \<preceq>\<^sup>* C''; P \<turnstile> C'' \<preceq>\<^sup>* C' \<rbrakk>
+  \<Longrightarrow> class P C'' = class P' C''"
+ by (drule classes_unchanged_set, simp)
+
+lemma classes_between_unchanged_subset:
+ "\<lbrakk> classes_between P C C' \<inter> classes_changed P P' = {} \<rbrakk>
+  \<Longrightarrow> classes_between P C C' \<subseteq> classes_between P' C C'"
+apply (frule classes_unchanged_set, simp)
+apply rule
+(* \<Rightarrow> *)
+apply clarify
+apply (cut_tac P = "\<lambda>x. P \<turnstile> x \<preceq>\<^sup>* C' \<longrightarrow> P' \<turnstile> C \<preceq>\<^sup>* x" in rtrancl_induct, simp+)
+ apply clarify
+ apply (subgoal_tac "P' \<turnstile> y \<prec>\<^sup>1 z")
+  prefer 2
+  apply (erule_tac x = y in allE, erule impE, force) apply (erule impE, force)
+  apply (drule same_class_same_superclass, simp, fastforce)
+ apply (erule impE, fastforce)
+ apply fastforce
+apply simp
+apply (cut_tac a = x and b = C' and P = "\<lambda>x. P \<turnstile> C \<preceq>\<^sup>* x \<longrightarrow> P' \<turnstile> x \<preceq>\<^sup>* C'" in converse_rtrancl_induct, simp+)
+ apply clarify
+ apply (subgoal_tac "P' \<turnstile> y \<prec>\<^sup>1 z")
+  prefer 2
+  apply (erule_tac x = y in allE, erule impE, force) apply (erule impE, force)
+  apply (drule same_class_same_superclass, simp, fastforce)
+ apply (erule impE, fastforce)
+ apply fastforce
+apply simp
+done
+
+lemma classes_between_unchanged_subcls:
+ "\<lbrakk> classes_between P C C' \<inter> classes_changed P P' = {}; P \<turnstile> C \<preceq>\<^sup>* C' \<rbrakk>
+   \<Longrightarrow> P' \<turnstile> C \<preceq>\<^sup>* C'"
+apply (drule classes_between_unchanged_subset)
+apply (force)
+done
+
+(* this direction requires a couple more assumptions *)
+lemma classes_between_unchanged_subset2:
+ "\<lbrakk> classes_between P C C' \<inter> classes_changed P P' = {}; P \<turnstile> C \<preceq>\<^sup>* C'; P' \<turnstile> C' \<preceq>\<^sup>* Object \<rbrakk>
+  \<Longrightarrow> classes_between P' C C' \<subseteq> classes_between P C C'"
+apply (frule classes_unchanged_set)
+apply clarify
+apply (cut_tac b = x and P = "\<lambda>x. P' \<turnstile> x \<preceq>\<^sup>* C' \<longrightarrow> P \<turnstile> C \<preceq>\<^sup>* x \<and> P \<turnstile> x \<preceq>\<^sup>* C'" in rtrancl_induct, simp+)
+ apply clarify
+ apply (erule impE, fastforce)
+ apply (metis (no_types, hide_lams) rtrancl.rtrancl_into_rtrancl rtrancl.rtrancl_refl 
+   same_class_same_superclass subcls1_confluent subcls_of_Obj_acyclic)
+apply simp
+done
+
+lemma classes_between_unchanged_subcls2:
+ "\<lbrakk> classes_between P C C' \<inter> classes_changed P P' = {};
+    P \<turnstile> C \<preceq>\<^sup>* C'; P' \<turnstile> C' \<preceq>\<^sup>* Object;
+    P' \<turnstile> C \<preceq>\<^sup>* C''; P' \<turnstile> C'' \<preceq>\<^sup>* C' \<rbrakk>
+   \<Longrightarrow> P \<turnstile> C \<preceq>\<^sup>* C''"
+apply (drule classes_between_unchanged_subset2, simp+)
+apply blast
+done
+
+lemma classes_between_unchanged_subcls3:
+ "\<lbrakk> classes_between P C C' \<inter> classes_changed P P' = {};
+    P \<turnstile> C \<preceq>\<^sup>* C'; P' \<turnstile> C' \<preceq>\<^sup>* Object;
+    P' \<turnstile> C \<preceq>\<^sup>* C''; P' \<turnstile> C'' \<preceq>\<^sup>* C' \<rbrakk>
+   \<Longrightarrow> P \<turnstile> C'' \<preceq>\<^sup>* C'"
+apply (drule classes_between_unchanged_subset2, simp+)
+apply blast
+done
+
+lemma classes_between_unchanged_same_set:
+ "\<lbrakk> classes_between P C C' \<inter> classes_changed P P' = {};
+    P \<turnstile> C \<preceq>\<^sup>* C'; P' \<turnstile> C' \<preceq>\<^sup>* Object \<rbrakk>
+  \<Longrightarrow> classes_between P C C' = classes_between P' C C'"
+apply rule
+ apply (rule classes_between_unchanged_subset, simp)
+apply (rule classes_between_unchanged_subset2, simp+)
+done
+
+lemma classes_between_classes_changed_sym:
+ "\<lbrakk> classes_between P C C' \<inter> classes_changed P P' = {};
+    P \<turnstile> C \<preceq>\<^sup>* C'; P' \<turnstile> C' \<preceq>\<^sup>* Object \<rbrakk>
+ \<Longrightarrow> classes_between P' C C' \<inter> classes_changed P' P = {}"
+apply (frule classes_between_unchanged_same_set, simp+)
+apply (cut_tac P = P and P' = P' in classes_changed_sym)
+apply simp
+done
+
+(*****************************Methods*********************************)
+
+
+(* HERE: is this an unnecessary special case of previous lemma? *)
+lemma classes_unchanged_sees_methods_exists:
+ "\<lbrakk> classes_between P C C' \<inter> classes_changed P P' = {}; P \<turnstile> C \<preceq>\<^sup>* C'; P' \<turnstile> C' \<preceq>\<^sup>* Object;
+     \<exists>D' fs ms. class P' Object = \<lfloor>(D', fs, ms)\<rfloor>;
+     P \<turnstile> C sees_methods Mm \<rbrakk>
+ \<Longrightarrow> \<exists>Mm. P' \<turnstile> C sees_methods Mm"
+apply (rule subcls_Obj_sees_methods_exists)
+apply (frule classes_between_unchanged_subcls, simp+)
+done
+
+
+lemma classes_between_do_not_see_methods:
+ "\<lbrakk> P \<turnstile> C sees_methods Mm; Mm M = Some(m,C'); D \<noteq> C'; D \<in> classes_between P C C' \<rbrakk>
+  \<Longrightarrow> \<exists>D' fs ms. class P D = Some(D',fs,ms) \<and> map_of ms M = None"
+apply clarsimp
+apply (cut_tac Pa = "\<lambda>C Mm. Mm M = \<lfloor>(m, C')\<rfloor> \<longrightarrow> P \<turnstile> C \<preceq>\<^sup>* D
+    \<longrightarrow> (\<exists>D' fs ms. class P D = \<lfloor>(D', fs, ms)\<rfloor> \<and> map_of ms M = None)"
+  in Methods.induct, simp)
+  apply clarify
+ apply clarify
+ apply (case_tac "Ca = D") apply simp
+ apply (erule disjE, clarsimp)
+  apply (subgoal_tac "P \<turnstile> D \<preceq>\<^sup>* Object")
+   prefer 2
+   apply (drule sees_methods_sub_Obj)
+   apply (rule subcls_of_Obj, simp+)
+  apply (drule subcls_of_Obj_acyclic, force, simp)
+ apply simp
+ apply (erule impE)
+  apply (drule_tac C = Ca in subcls1I, simp)
+  apply (simp add: subcls1_confluent)
+ apply simp
+apply simp
+done
+
+(* Important! *)
+lemma classes_unchanged_sees_method_same:
+ "\<lbrakk> classes_between P C C' \<inter> classes_changed P P' = {}; P \<turnstile> C sees_methods Mm;
+     P' \<turnstile> C sees_methods Mm'; Mm M = Some(m,C') \<rbrakk>
+  \<Longrightarrow> Mm' M = Some(m,C')"
+apply (frule sees_methods_decl_above, simp)
+apply (frule classes_between_unchanged_subcls, simp)
+apply (cut_tac a = C and b = C' and
+  P = "\<lambda>C''. \<forall>Mm Mm'. P \<turnstile> C \<preceq>\<^sup>* C'' \<longrightarrow> P \<turnstile> C'' sees_methods Mm \<longrightarrow>
+           P' \<turnstile> C'' sees_methods Mm' \<longrightarrow>
+           Mm M = \<lfloor>(m, C')\<rfloor> \<longrightarrow> Mm' M = \<lfloor>(m, C')\<rfloor>" in converse_rtrancl_induct, simp)
+  apply clarsimp
+  apply (drule_tac Mm = Mma in visible_methods_exist, simp, clarsimp)
+  apply (drule classes_between_unchanged, simp+)
+  apply (rule_tac ?a2.0 = Mm'a in Methods.cases, simp+)
+ apply clarsimp
+ apply (drule_tac D = y in classes_between_do_not_see_methods, simp)
+   apply (metis (no_types, lifting) r_into_rtrancl sees_methods_sub_Obj subcls1D subcls_of_Obj_acyclic subcls_self_superclass)
+  apply simp
+ apply (drule_tac C'' = y in classes_between_unchanged, simp+)
+ apply (frule subcls1D, clarsimp)
+ apply (erule impE) apply auto[1]
+ apply (rule_tac ?a2.0 = Mma in Methods.cases, simp+)
+ apply (rule_tac ?a2.0 = Mm'a in Methods.cases, simp+)
+ apply (erule_tac x = Mmaa in allE, erule impE, simp)
+ apply (erule_tac x = Mmb in allE, erule impE, simp)
+ apply (erule impE) apply auto[1]
+ apply (simp add: map_add_Some_iff)
+apply simp
+done
+
+lemma classes_unchanged_sees_same_method:
+ "\<lbrakk> classes_between P C C' \<inter> classes_changed P P' = {};
+     P' \<turnstile> C' \<preceq>\<^sup>* Object; \<exists>D' fs ms. class P' Object = \<lfloor>(D', fs, ms)\<rfloor>;
+     P \<turnstile> C sees M,b: Ts\<rightarrow>T = m in C' \<rbrakk>
+  \<Longrightarrow> P' \<turnstile> C sees M,b: Ts\<rightarrow>T = m in C'"
+apply (frule sees_method_decl_above)
+apply (clarsimp simp add: Method_def)
+apply (frule classes_unchanged_sees_methods_exists, simp+)
+apply (clarify, rule_tac x = Mma in exI, simp)
+apply (rule classes_unchanged_sees_method_same, simp+)
+done
+
+
+lemma classes_unchanged_sees_same_method2:
+ "\<lbrakk> classes_between P C C' \<inter> classes_changed P P' = {};
+     P \<turnstile> C \<preceq>\<^sup>* C'; P \<turnstile> C' \<preceq>\<^sup>* Object; \<exists>D' fs ms. class P Object = \<lfloor>(D', fs, ms)\<rfloor>;
+     P' \<turnstile> C sees M,b: Ts\<rightarrow>T = m in C' \<rbrakk>
+  \<Longrightarrow> P \<turnstile> C sees M,b: Ts\<rightarrow>T = m in C'"
+apply (frule sees_method_decl_above)
+apply (drule classes_between_classes_changed_sym, simp+)
+ apply (meson Method_def sees_methodsD subcls_of_Obj)
+apply (rule classes_unchanged_sees_same_method, simp+)
+done
+
+
+(********************* Fields ************************)
+
+(* HERE: is this an unnecessary special case of previous lemma? *)
+lemma classes_unchanged_has_fields_exists:
+ "\<lbrakk> classes_between P C C' \<inter> classes_changed P P' = {}; P \<turnstile> C \<preceq>\<^sup>* C'; P' \<turnstile> C' \<preceq>\<^sup>* Object;
+     \<exists>D' fs ms. class P' Object = \<lfloor>(D', fs, ms)\<rfloor>;
+     P \<turnstile> C has_fields FDTs \<rbrakk>
+ \<Longrightarrow> \<exists>FDTs. P' \<turnstile> C has_fields FDTs"
+apply (rule subcls_Obj_has_fields_exists)
+apply (frule classes_between_unchanged_subcls, simp+)
+done
+
+
+lemma classes_between_do_not_see_fields:
+ "\<lbrakk> P \<turnstile> C has_fields FDTs; map_of (map (\<lambda>((F,D),b,T). (F,(D,b,T))) FDTs) F = Some(C',b,T);
+     D \<noteq> C'; D \<in> classes_between P C C' \<rbrakk>
+  \<Longrightarrow> \<exists>D' fs ms. class P D = Some(D',fs,ms) \<and> map_of fs F = None"
+apply clarsimp
+apply (cut_tac
+  Pa = "\<lambda>C FDTs. map_of (map (\<lambda>((F,D),b,T). (F,(D,b,T))) FDTs) F = Some(C',b,T) \<longrightarrow>
+    P \<turnstile> C \<preceq>\<^sup>* D \<longrightarrow> (\<exists>D' fs ms. class P D = \<lfloor>(D', fs, ms)\<rfloor> \<and> map_of fs F = None)"
+  in Fields.induct, simp)
+   prefer 2 apply clarify
+ apply (subgoal_tac "map_of (map ((\<lambda>((F, D), b, T). (F, D, b, T)) \<circ> (\<lambda>(F, y). ((F, Ca), y))) fs)
+   = map_of (map (\<lambda>(F, y). (F, Ca, y)) fs)")
+  prefer 2
+  apply (simp add: map_of_remap_insertmap)
+ apply clarsimp
+ apply (case_tac "Ca = D", clarsimp)
+  apply (erule disjE)
+   apply (drule map_of_insertmap_Some_eq, simp)
+  apply (clarify, drule map_of_insertmap_NoneD, simp)
+ apply (erule disjE)
+  apply (drule map_of_insertmap_Some_eq)
+  apply (subgoal_tac "P \<turnstile> D \<preceq>\<^sup>* Object")
+   prefer 2
+   apply (drule has_fields_sub_Obj)
+   apply (rule subcls_of_Obj, simp+)
+  apply (drule subcls_of_Obj_acyclic, force, simp)
+ apply simp
+ apply (erule impE)
+  apply (drule_tac C = Ca in subcls1I, simp)
+  apply (simp add: subcls1_confluent)
+ apply simp
+apply simp
+done
+
+(* Important! *)
+lemma classes_unchanged_has_field_same:
+ "\<lbrakk> classes_between P C C' \<inter> classes_changed P P' = {}; P \<turnstile> C has_fields FDTs;
+     P' \<turnstile> C has_fields FDTs'; map_of (map (\<lambda>((F,D),b,T). (F,(D,b,T))) FDTs) F = Some(C',b,T) \<rbrakk>
+  \<Longrightarrow> map_of (map (\<lambda>((F,D),b,T). (F,(D,b,T))) FDTs') F = Some(C',b,T)"
+apply (frule_tac F = F and D = C' and b = b and T = T in has_fields_decl_above)
+ apply (simp add: map_of_SomeD map_of_remap_SomeD2)
+apply (frule classes_between_unchanged_subcls, simp)
+apply (cut_tac a = C and b = C' and
+  P = "\<lambda>C''. \<forall>FDTs FDTs'. P \<turnstile> C \<preceq>\<^sup>* C'' \<longrightarrow> P \<turnstile> C'' has_fields FDTs \<longrightarrow>
+           P' \<turnstile> C'' has_fields FDTs' \<longrightarrow>
+           map_of (map (\<lambda>((F,D),b,T). (F,(D,b,T))) FDTs) F = Some(C',b,T) \<longrightarrow>
+           map_of (map (\<lambda>((F,D),b,T). (F,(D,b,T))) FDTs') F = Some(C',b,T)"
+      in converse_rtrancl_induct, simp)
+  apply clarsimp
+  apply (drule_tac FDTs = FDTsa and F = F and D = C' and b = b and T = T
+    in visible_fields_exist)
+   apply (simp add: map_of_remap_SomeD2, clarsimp)
+  apply (drule classes_between_unchanged, simp+)
+  apply (rule_tac ?a2.0 = FDTs'a in Fields.cases, simp+)
+    apply (clarsimp simp add: map_add_def, rule conjI)
+     apply (metis map_of_insertmap_NoneD map_of_remap_insertmap option.distinct(1))
+    apply (clarsimp simp add: map_of_remap_insertmap)
+    apply (drule_tac D = C' in map_of_insertmap_SomeD2', fastforce)
+   apply (clarsimp simp add: map_of_remap_insertmap)
+   apply (drule_tac D = C' in map_of_insertmap_SomeD2', fastforce)
+ apply clarsimp
+ apply (drule_tac D = y in classes_between_do_not_see_fields, simp)
+   apply (metis (no_types, lifting) has_fields_sub_Obj r_into_rtrancl subcls1D subcls_of_Obj_acyclic subcls_self_superclass)
+  apply simp
+ apply (drule_tac C'' = y in classes_between_unchanged, simp+)
+ apply (frule subcls1D, clarsimp)
+ apply (erule impE) apply auto[1]
+ apply (rule_tac ?a2.0 = FDTsa in Fields.cases, simp+)
+  apply (clarsimp simp add: map_of_remap_insertmap)
+  apply (erule disjE)
+   apply (drule_tac fs = fsa and D = Ca in map_of_insertmap_NoneD', fastforce)
+  apply clarify
+  apply (cut_tac P = P' and C = z in subcls_Obj_has_fields_exists)
+    apply (meson has_fields_sub_Obj subcls1.subcls1I subcls1_confluent)
+   using has_fieldsD apply blast
+  apply (erule_tac x = FDTsa in allE, clarsimp, erule_tac x = FDTsb in allE, simp)
+  apply (drule_tac P = P' and C = Ca in has_fields_rec, simp+)
+  apply (drule has_fields_fun, simp, clarsimp)
+  apply (clarsimp simp add: map_add_def, rule conjI)
+   apply (metis map_of_remap_insertmap option.distinct(1))
+  apply (clarsimp simp add: map_of_remap_insertmap)
+ apply (drule_tac D = C' in map_of_insertmap_SomeD2', fastforce)
+ apply (clarsimp simp add: map_of_remap_insertmap)
+done
+
+
+lemma classes_unchanged_sees_same_field:
+ "\<lbrakk> classes_between P C C' \<inter> classes_changed P P' = {};
+    P' \<turnstile> C' \<preceq>\<^sup>* Object; \<exists>D' fs ms. class P' Object = \<lfloor>(D', fs, ms)\<rfloor>;
+    P \<turnstile> C sees F,b:t in C' \<rbrakk>
+   \<Longrightarrow> P' \<turnstile> C sees F,b:t in C'"
+apply (frule sees_field_decl_above)
+apply (clarsimp simp add: sees_field_def)
+apply (frule classes_unchanged_has_fields_exists, simp+)
+apply (clarify, rule_tac x = FDTsa in exI, simp)
+apply (rule classes_unchanged_has_field_same, simp+)
+done
+
+
+lemma classes_unchanged_sees_same_field2:
+ "\<lbrakk> classes_between P C C' \<inter> classes_changed P P' = {};
+     P \<turnstile> C \<preceq>\<^sup>* C'; P \<turnstile> C' \<preceq>\<^sup>* Object; \<exists>D' fs ms. class P Object = \<lfloor>(D', fs, ms)\<rfloor>;
+    P' \<turnstile> C sees F,b:t in C' \<rbrakk>
+   \<Longrightarrow> P \<turnstile> C sees F,b:t in C'"
+apply (frule sees_field_decl_above)
+apply (drule classes_between_classes_changed_sym, simp+)
+ apply (meson has_fieldsD sees_field_def subcls_of_Obj)
+apply (rule classes_unchanged_sees_same_field, simp+)
+done
+
+
+(***********************************
+(* overrides *)
+
+
+lemma classes_unchanged_closest_above_same:
+ "\<lbrakk> classes_between P C' D \<inter> classes_changed P P' = {};
+    P \<turnstile> C sees M,b:Ts \<rightarrow> T = m in D; P \<turnstile> C' \<preceq>\<^sup>* C;
+    P \<turnstile> C' \<preceq>\<^sup>* C''; P' \<turnstile> D \<preceq>\<^sup>* Object; \<exists>D' fs ms. class P' Object = \<lfloor>(D', fs, ms)\<rfloor>;
+    P \<turnstile> C'' closestAbove C' that (\<lambda>P C''. \<exists>m' D'. P \<turnstile> C'' sees M,b :  Ts\<rightarrow>T = m' in D') \<rbrakk>
+ \<Longrightarrow>
+    P' \<turnstile> C'' closestAbove C' that (\<lambda>P C''. \<exists>m' D'. P \<turnstile> C'' sees M,b :  Ts\<rightarrow>T = m' in D')"
+apply (clarsimp simp add: Closest_above_that_def)
+
+apply (subgoal_tac "P \<turnstile> C'' \<preceq>\<^sup>* C")
+ prefer 2
+ apply (erule_tac x = C in allE, erule impE, simp, blast)
+ apply simp
+
+apply (subgoal_tac "P \<turnstile> C'' \<preceq>\<^sup>* D")
+ prefer 2
+ apply (rule_tac y = C in rtrancl_trans, simp)
+ apply (rule sees_method_decl_above, simp)
+
+apply (subgoal_tac "P' \<turnstile> C' \<preceq>\<^sup>* C''")
+ prefer 2
+ apply (rule_tac P = P in classes_between_unchanged_subcls)
+  apply (rule subset_empty_intersect, simp)
+  apply (rule classes_between_subset_below, simp)
+  apply simp
+ apply simp
+
+apply (subgoal_tac "P \<turnstile> C'' \<preceq>\<^sup>* D'a")
+ prefer 2
+ apply (rule sees_method_decl_above, simp)
+
+apply (subgoal_tac "P \<turnstile> D'a \<preceq>\<^sup>* D")
+ prefer 2
+ apply (rule sees_method_decl_mono, simp_all)
+
+apply (subgoal_tac "classes_between P D'a D \<inter> classes_changed P P' = {}")
+ prefer 2
+ apply (rule subset_empty_intersect, simp)
+ apply (rule classes_between_subset_between, simp+)
+
+apply (subgoal_tac "P' \<turnstile> D'a \<preceq>\<^sup>* D")
+ prefer 2
+ apply (rule_tac P = P in classes_between_unchanged_subcls, simp+)
+
+apply (subgoal_tac "P' \<turnstile> D'a \<preceq>\<^sup>* Object")
+ prefer 2
+ apply (rule rtrancl_trans, simp+)
+
+apply (subgoal_tac "classes_between P C'' D'a \<inter> classes_changed P P' = {}")
+ prefer 2
+ apply (rule subset_empty_intersect, simp)
+ apply (rule classes_between_subset_between, simp+)
+
+apply (subgoal_tac "P' \<turnstile> C'' sees M :  Ts\<rightarrow>T = m' in D'a, static b")
+ prefer 2
+ apply (rule_tac P = P in classes_unchanged_sees_same_method, simp+)
+
+apply (subgoal_tac "classes_between P C' C'' \<inter> classes_changed P P' = {}")
+ prefer 2
+ apply (rule subset_empty_intersect, simp)
+ apply (rule classes_between_subset_below, simp+)
+
+apply (subgoal_tac "P' \<turnstile> C'' \<preceq>\<^sup>* D")
+ prefer 2
+ apply (rule_tac P = P in classes_between_unchanged_subcls)
+  apply (rule subset_empty_intersect, simp)
+  apply (rule classes_between_subset_above, simp)
+  apply simp
+ apply simp
+
+apply (subgoal_tac "P' \<turnstile> C'' \<preceq>\<^sup>* Object")
+ prefer 2
+ apply (rule rtrancl_trans, simp+)
+
+apply (subgoal_tac "\<forall>C''a. P' \<turnstile> C' \<preceq>\<^sup>* C''a \<and>
+  (\<exists>m' D'. P' \<turnstile> C''a sees M :  Ts\<rightarrow>T = m' in D', static b) \<longrightarrow> P' \<turnstile> C'' \<preceq>\<^sup>* C''a")
+ prefer 2
+ apply clarsimp
+ apply (frule_tac P = P' and C' = C'' and C'' = C''a in subcls_confluent, assumption, erule disjE)
+  apply simp
+
+ apply (subgoal_tac "P \<turnstile> C' \<preceq>\<^sup>* C''a")
+  prefer 2
+  apply (rule_tac C' = C'' in classes_between_unchanged_subcls2, simp+)
+
+ apply (subgoal_tac "P' \<turnstile> D'b \<preceq>\<^sup>* D'a")
+  prefer 2
+  apply (rule_tac P = P' and C = C'' and C' = C''a in sees_method_decl_mono, simp+)
+
+ apply (subgoal_tac "P' \<turnstile> D'b \<preceq>\<^sup>* D")
+  prefer 2
+  apply (rule_tac y = D'a in rtrancl_trans, simp+)
+
+ apply (subgoal_tac "P' \<turnstile> C''a \<preceq>\<^sup>* D'b")
+  prefer 2
+  apply (rule sees_method_decl_above, simp)
+
+ apply (subgoal_tac "P' \<turnstile> C' \<preceq>\<^sup>* D'b")
+  prefer 2
+  apply (rule_tac y = C''a in rtrancl_trans, simp+)
+
+ apply (subgoal_tac "P \<turnstile> C' \<preceq>\<^sup>* D'b")
+  prefer 2
+  apply (rule classes_between_unchanged_subcls2, simp+)
+
+ apply (subgoal_tac "P \<turnstile> D'b \<preceq>\<^sup>* D")
+  prefer 2
+  apply (rule classes_between_unchanged_subcls3, simp+)
+
+ apply (subgoal_tac "classes_between P C' D'b \<inter> classes_changed P P' = {}")
+  prefer 2
+  apply (rule subset_empty_intersect, simp)
+  apply (rule classes_between_subset_below, simp+)
+
+ apply (subgoal_tac "P \<turnstile> C''a \<preceq>\<^sup>* D'b")
+  prefer 2
+  apply (rule classes_between_unchanged_subcls3, simp+)
+
+ apply (subgoal_tac "classes_between P C''a D'b \<inter> classes_changed P P' = {}")
+  prefer 2
+  apply (rule_tac R = "classes_between P C' D'b" in subset_empty_intersect, simp)
+  apply (rule classes_between_subset_above, simp+)
+
+ apply (subgoal_tac "P \<turnstile> D'b \<preceq>\<^sup>* Object")
+  prefer 2
+  apply (meson rtrancl_trans sees_method_sub_Obj subcls_of_Obj)
+
+ apply (subgoal_tac "\<exists>D' fs ms. class P Object = \<lfloor>(D', fs, ms)\<rfloor>")
+  prefer 2
+  apply (rule sees_method_Object_exists, simp)
+
+ apply (subgoal_tac "P \<turnstile> C''a sees M :  Ts\<rightarrow>T = m'a in D'b, static b")
+  prefer 2
+  apply (rule_tac P' = P' in classes_unchanged_sees_same_method2, simp+)
+
+ apply (subgoal_tac "P \<turnstile> C''a \<preceq>\<^sup>* C''")
+  prefer 2
+  apply (rule classes_between_unchanged_subcls3, simp+)
+
+ apply (erule_tac x = C''a in allE)
+ apply (erule impE, simp, blast)
+ apply (subgoal_tac "C'' = C''a")
+  prefer 2
+  apply (meson sees_method_sub_Obj subcls_of_Obj_acyclic)
+ apply simp
+apply blast
+done
+
+
+lemma classes_unchanged_overrides_same:
+ "\<lbrakk> classes_between P C' D \<inter> classes_changed P P' = {};
+    P' \<turnstile> D \<preceq>\<^sup>* Object; \<exists>D' fs ms. class P' Object = \<lfloor>(D', fs, ms)\<rfloor>;
+    P \<turnstile> C', m', D' overrides C, M = m in D : Ts \<rightarrow> T, static b \<rbrakk>
+ \<Longrightarrow> P' \<turnstile> C', m', D' overrides C, M = m in D : Ts \<rightarrow> T, static b"
+apply (frule overrides_subcls)
+apply (clarsimp simp add: Overrides_def)
+
+apply (subgoal_tac "P' \<turnstile> C sees M :  Ts\<rightarrow>T = m in D, static b")
+ prefer 2
+ apply (rule classes_unchanged_sees_same_method, simp_all)
+   apply (frule subset_empty_intersect, rule_tac C' = C in classes_between_subset_above)
+   apply (simp, rule sees_method_decl_above, simp+)
+
+apply (subgoal_tac "P \<turnstile> C' \<preceq>\<^sup>* C''")
+ prefer 2
+ apply (rule closest_above_subcls, simp)
+
+apply (subgoal_tac "classes_between P C'' C \<inter> classes_changed P P' = {}")
+ prefer 2
+ apply (rule subset_empty_intersect, simp)
+  apply (rule classes_between_subset_between, simp+)
+ apply (rule sees_method_decl_above, simp)
+
+apply (subgoal_tac "P' \<turnstile> C'' \<preceq>\<^sup>* C")
+ prefer 2
+ apply (rule_tac P = P in classes_between_unchanged_subcls, simp+)
+
+apply (subgoal_tac "P \<turnstile> C'' \<preceq>\<^sup>* D'")
+ prefer 2
+ apply (rule sees_method_decl_above, simp)
+
+apply (subgoal_tac "P \<turnstile> D' \<preceq>\<^sup>* D")
+ prefer 2
+ apply (rule_tac C' = C'' in sees_method_decl_mono, simp+)
+
+apply (subgoal_tac "classes_between P C'' D' \<inter> classes_changed P P' = {}")
+ prefer 2
+ apply (rule subset_empty_intersect, simp)
+  apply (rule classes_between_subset_between, simp+)
+
+apply (subgoal_tac "classes_between P D' D \<inter> classes_changed P P' = {}")
+ prefer 2
+ apply (rule subset_empty_intersect, simp)
+  apply (rule classes_between_subset_above, simp+)
+
+apply (subgoal_tac "P' \<turnstile> D' \<preceq>\<^sup>* D")
+ prefer 2
+ apply (rule_tac P = P in classes_between_unchanged_subcls, simp+)
+
+apply (subgoal_tac "P' \<turnstile> D' \<preceq>\<^sup>* Object")
+ prefer 2
+ apply (rule rtrancl_trans, simp+)
+
+apply (subgoal_tac "P' \<turnstile> C'' sees M :  Ts\<rightarrow>T = m' in D', static b")
+ prefer 2
+ apply (rule_tac P = P in classes_unchanged_sees_same_method, simp+)
+
+apply (subgoal_tac "P' \<turnstile> C'' closestAbove C' that (\<lambda>P C''. \<exists>m' D'. P \<turnstile> C'' sees M :  Ts\<rightarrow>T = m' in D', static b)")
+ prefer 2
+ apply (rule classes_unchanged_closest_above_same, simp+)
+
+apply blast
+done
+
+***********************************************)
+
+(* HERE: move this when done *)
+(* not currently used *)
+lemma cyclic_implies:
+ "\<lbrakk> P \<turnstile> C \<preceq>\<^sup>* C'; P \<turnstile> C' \<preceq>\<^sup>* C; C \<noteq> C' \<rbrakk>
+\<Longrightarrow> \<forall>x. P \<turnstile> C \<preceq>\<^sup>* x \<longrightarrow> P \<turnstile> x \<preceq>\<^sup>* C"
+apply clarify
+apply (frule_tac b = x and P = "\<lambda>x. P \<turnstile> C \<preceq>\<^sup>* x \<longrightarrow> P \<turnstile> x \<preceq>\<^sup>* C'" in rtrancl_induct, simp)
+ apply clarsimp
+ apply (case_tac "y = C'")
+  apply (metis rtrancl_trans subcls1_confluent)
+ apply (simp add: subcls1_confluent)
+apply simp
+done
+
+(* HERE: below is currently unused, but may need it in the future *)
+(*
+(* is this true? trying to find a way to obtain the new acyclicity assumption using simpler
+  assumptions *)
+lemma
+ "\<lbrakk> P \<turnstile> C \<preceq>\<^sup>* Object \<longrightarrow> P' \<turnstile> C \<preceq>\<^sup>* Object (*;
+    P' cyclicAbove C' \<longrightarrow> P cyclicAbove C' *) \<rbrakk>
+\<Longrightarrow> (* NO - not enough *)
+   \<forall>C'. P \<turnstile> C \<preceq>\<^sup>* C' \<and> P' \<turnstile> C \<preceq>\<^sup>* C' \<and> P' \<turnstile> C' \<preceq>\<^sup>* C \<longrightarrow> P \<turnstile> C' \<preceq>\<^sup>* C"
+apply clarsimp
+apply (case_tac "C = C'", simp)
+apply (case_tac "P \<turnstile> C \<preceq>\<^sup>* Object")
+ apply simp
+ apply (drule subcls_of_Obj_acyclic, simp)+
+ apply simp
+apply simp
+thm subcls_of_Obj_acyclic subcls_of_Obj_acyclic1
+find_theorems name:acyclic
+oops
+*)
+
+(* this direction requires an acyclicity assumption *)
+(* we were attempting to modify the assumption used, but for now we'll stick with what we have below *)
+(*
+lemma classes_between_unchanged_subset2:
+ "\<lbrakk> classes_between P C C' \<inter> classes_changed P P' = {}; P \<turnstile> C \<preceq>\<^sup>* C';
+(*    \<forall>C''. P \<turnstile> C' \<preceq>\<^sup>* C'' \<and> P' \<turnstile> C' \<preceq>\<^sup>* C'' \<and> P' \<turnstile> C'' \<preceq>\<^sup>* C' \<longrightarrow> P \<turnstile> C'' \<preceq>\<^sup>* C' (* i.e., acyclicity has not been introduced *)*)
+    P' cyclicAbove C' \<longrightarrow> P cyclicAbove C' \<rbrakk>
+  \<Longrightarrow> classes_between P' C C' \<subseteq> classes_between P C C'"
+apply (frule classes_unchanged_set)
+apply clarify
+apply (cut_tac b = x and P = "\<lambda>x. P' \<turnstile> C \<preceq>\<^sup>* x \<and> P' \<turnstile> x \<preceq>\<^sup>* C' \<longrightarrow> P \<turnstile> C \<preceq>\<^sup>* x \<and> P \<turnstile> x \<preceq>\<^sup>* C'" in rtrancl_induct, simp+)
+ apply clarify
+ apply (erule impE, fastforce)
+(* apply (subgoal_tac "P \<turnstile> y \<prec>\<^sup>1 z")
+  prefer 2
+  apply (metis (no_types, lifting) same_class_same_superclass) *)
+ (****)
+ defer
+ apply (metis (no_types, lifting) cyclic_above_def rtrancl.rtrancl_into_rtrancl subcls1_confluent subcls_confluent
+apply simp
+oops
+(**)
+apply (case_tac "P' cyclicAbove C'", simp)
+ apply (clarsimp simp add: cyclic_above_def) defer
+apply simp
+apply (subgoal_tac "P \<turnstile> y \<prec>\<^sup>1 z")
+ prefer 2
+ apply (metis (no_types, lifting) same_class_same_superclass)
+done
+*)
+
+end
