Common/ClassesChanged.thy
@@ -1,0 +1,172 @@
+(*  Title:      Jinja/Common/ClassesChanged.thy
+    Author:    Susannah Mansky, UIUC 2016
+*)
+
+(* HERE: write a better .thy description *)
+section {* Theory around the classes changed from one program to another, and how
+  if classes are not changed, the same things are visible in those classes *}
+
+theory ClassesChanged
+imports "../MapOfThy" "../SupplSetThy" Exceptions
+begin
+
+(***)
+
+(* a class is considered changed if it exists only in one program or the other,
+  or exists in both but is different *)
+definition classes_changed :: "'m prog \<Rightarrow> 'm prog \<Rightarrow> cname set" where
+"classes_changed P1 P2
+   = foldl (\<lambda>a (cn, c). if class P1 cn \<noteq> class P2 cn then insert cn a else a) {} (P1@P2)"
+(*"classes_changed P1 P2 = {cn. class P1 cn \<noteq> class P2 cn}"*)
+
+lemma classes_changed_equiv:
+ "cn \<in> classes_changed P1 P2
+   = ((class P1 cn \<noteq> class P2 cn) \<and> (\<exists>x. fst x = cn \<and> x \<in> set (P1@P2)))"
+apply (simp only: classes_changed_def class_def)
+apply (cut_tac f = "fst" and y = "(cn, the (map_of P2 cn))" and s = "{}" and
+  ?l2.0 = "P1@P2" and P = "\<lambda>x. map_of P1 x \<noteq> map_of P2 x" in foldl_if_insert)
+apply (subgoal_tac "\<forall>l s. (foldl (\<lambda>a (cn, c). if map_of P1 cn \<noteq> map_of P2 cn then insert cn a else a) s l =
+foldl (\<lambda>a x. if map_of P1 (fst x) \<noteq> map_of P2 (fst x) then insert (fst x) a else a) s l)")
+ prefer 2
+ apply (clarify, rule list.induct, simp)
+ apply (meson foldl_cong prod.case_eq_if)
+apply (erule_tac x = "P1@P2" in allE, erule_tac x = "{}" in allE, clarsimp)
+done
+
+lemma classes_changed_exists:
+  "cn \<in> classes_changed P1 P2 \<Longrightarrow> class P1 cn \<noteq> None \<or> class P2 cn \<noteq> None"
+apply (simp only: classes_changed_equiv, erule conjE)
+apply (simp only: class_exists_equiv2)
+done
+
+
+definition class_changed :: "'m prog \<Rightarrow> 'm prog \<Rightarrow> cname \<Rightarrow> bool" where
+"class_changed P1 P2 cn = (class P1 cn \<noteq> class P2 cn)"
+
+lemma class_changed_exists:
+  "class_changed P1 P2 cn \<Longrightarrow> class P1 cn \<noteq> None \<or> class P2 cn \<noteq> None"
+apply (simp add: class_changed_def)
+apply (rule classical)
+apply (subgoal_tac "class P1 cn = None \<and> class P2 cn = None")
+ prefer 2
+ apply force
+apply simp
+done
+
+lemma classes_changed_class_changed[simp]: "cn \<in> classes_changed P1 P2 = class_changed P1 P2 cn"
+apply (simp add: classes_changed_equiv)
+apply (rule iffI)
+ apply (simp add: class_changed_def)
+apply (frule class_changed_exists)
+apply (simp add: class_changed_def class_def)
+apply (meson map_of_SomeD)
+done
+
+lemma classes_changed_self[simp]: "classes_changed P P = {}"
+ by (auto simp add: class_changed_def)
+
+lemma classes_changed_sym: "classes_changed P P' = classes_changed P' P"
+ by (auto simp add: class_changed_def)
+
+lemma class_changed_equiv:
+ "class_changed P1 P2 cn =
+   ((class P1 cn \<noteq> class P2 cn) \<and> (class P1 cn \<noteq> None \<or> class P2 cn \<noteq> None))"
+apply (simp only: classes_changed_class_changed [THEN sym] classes_changed_equiv class_exists_equiv2)
+done
+
+
+(* lemma relating classes_changed to execution changes, or lack thereof *)
+lemma classes_changed_nin_same: "\<lbrakk> cn \<notin> classes_changed P P'\<rbrakk> \<Longrightarrow> class P cn = class P' cn"
+apply (clarsimp simp add: class_changed_equiv)
+by (metis option.exhaust prod_cases3)
+
+lemma classes_unchanged_set: "\<lbrakk> S \<inter> classes_changed P P' = {} \<rbrakk>
+  \<Longrightarrow> \<forall>C \<in> S. class P C = class P' C"
+apply (clarsimp simp add: disjoint_iff_not_equal)
+apply (rule classes_changed_nin_same, force)
+done
+
+(** Program structure lemmas **)
+
+lemma class_changed_singleton:
+ "class_changed [t] P' (fst t) \<Longrightarrow> class_changed (t # P) P' (fst t)"
+ by (simp add: class_changed_def class_def)
+
+lemma class_changed_singleton2:
+ "class_changed P [t] (fst t) \<Longrightarrow> class_changed P (t # P') (fst t)"
+ by (simp add: class_changed_def class_def)
+
+lemma not_class_changed_singleton:
+ "\<not> class_changed [t] P' (fst t) \<Longrightarrow> fst t \<notin> classes_changed (t # P) P'"
+apply simp
+apply (rule classical, simp)
+apply (erule notE, simp add: class_changed_def class_def)
+done
+
+(* HERE: might want to change next few lemmas slightly; they work as is for now *)
+lemma classes_changed_cons_changed_subset:
+ "class_changed [t] P' (fst t) \<Longrightarrow> classes_changed P P' \<subseteq> classes_changed (t # P) P'"
+by (smt class_changed_singleton class_cons classes_changed_class_changed classes_changed_equiv
+  classes_changed_nin_same subsetI)
+
+lemma classes_unchanged_cons_changed_subset:
+"\<not> class_changed [t] P' (fst t) \<Longrightarrow> classes_changed P P' - {fst t} \<subseteq> classes_changed (t # P) P'"
+by (smt DiffE class_cons classes_changed_equiv classes_changed_nin_same insertCI subsetI)
+
+lemma classes_unchanged_cons_changed_subset2:
+ "\<not> class_changed [t] P' (fst t) \<Longrightarrow> classes_changed (t # P) P' \<subseteq> classes_changed P P'"
+apply (frule_tac P = P in not_class_changed_singleton)
+apply (metis class_cons classes_changed_equiv classes_changed_nin_same subsetI)
+done
+
+lemma classes_changed_cons:
+ "classes_changed (t # P) P' = (classes_changed P P' - {fst t})
+                     \<union> (if class_changed [t] P' (fst t) then {fst t} else {})"
+apply (case_tac "class_changed [t] P' (fst t)")
+ apply simp
+ apply rule
+  apply (metis class_cons classes_changed_equiv classes_changed_nin_same insertCI subsetI)
+ apply (rule insert_subsetI)
+  apply (drule class_changed_singleton, simp)
+  apply (rule classes_changed_cons_changed_subset, simp)
+apply simp
+apply rule
+ apply (rule not_in_Diff_subsetI)
+  apply (rule classes_unchanged_cons_changed_subset2, simp)
+  apply (cut_tac not_class_changed_singleton, simp+)
+apply (rule classes_unchanged_cons_changed_subset, simp)
+done
+
+
+lemma class_changed_same_cons:
+ "fst t \<notin> classes_changed (t#P) (t#P')"
+ by (simp add: class_changed_def class_def)
+
+lemma classes_changed_same_cons:
+ "classes_changed (t # P) (t # P') = classes_changed P P' - {fst t}"
+proof(cases "fst t \<in> classes_changed P P'")
+  case True
+  then show ?thesis using class_changed_same_cons[where t=t and P=P and P'=P']
+    classes_changed_cons[where t=t] by (auto simp: class_changed_def class_cons)
+next
+  case False
+  then show ?thesis using class_changed_same_cons[where t=t and P=P and P'=P']
+    by (auto simp: class_changed_def) (metis (no_types, lifting) class_cons)+
+qed
+
+lemma classes_changed_int_Cons:
+assumes "coll \<inter> classes_changed P P' = {}"
+shows "coll \<inter> classes_changed (t # P) (t # P') = {}"
+proof(cases "fst t \<in> classes_changed P P'")
+  case True
+  then have "classes_changed P P' = classes_changed (t # P) (t # P') \<union> {fst t}"
+    using classes_changed_same_cons[where t=t and P=P and P'=P'] by fastforce
+  then show ?thesis using assms by simp
+next
+  case False
+  then have "classes_changed P P' = classes_changed (t # P) (t # P')"
+    using classes_changed_same_cons[where t=t and P=P and P'=P'] by fastforce
+  then show ?thesis using assms by simp
+qed
+
+end
