JinjaDCI.thy
@@ -3,6 +3,7 @@ imports
   "J/Equivalence"
   "J/Annotate"
   "BV/TF_JVM"
+  "BV/BVNoTypeError"
   "Compiler/TypeComp"
 begin
 
